Do some manual inlining

quotation/theories/ToPCUIC/Init/Typing.v
@@ -1,3 +1,948 @@
+From MetaCoq.Utils Require Import utils monad_utils MCList.
+From MetaCoq.Common Require Import Kernames MonadBasicAst.
+From MetaCoq.Template Require MonadAst TemplateMonad Ast Loader.
+Require Import Equations.Prop.Classes.
+Require Import Coq.Lists.List.
+Import ListNotations.
+
+Local Unset Universe Minimization ToSet.
+Local Set Primitive Projections.
+Local Open Scope bs.
+Import MCMonadNotation.
+
+Class debug_opt := debug : bool.
+Class cls_is_true (b : bool) := is_truev : is_true b.
+
+(* returns true if a modpath is suitable for quotation, i.e., does not mention functor-bound arguments *)
+Fixpoint modpath_is_absolute (mp : modpath) : bool
+  := match mp with
+     | MPfile _ => true
+     | MPbound _ _ _ => false
+     | MPdot mp _ => modpath_is_absolute mp
+     end.
+Definition kername_is_absolute (kn : kername) : bool
+  := modpath_is_absolute (fst kn).
+(* gives the dirpath and the reversed list of idents, or None if bound *)
+Fixpoint split_common_prefix_ls (mp1 mp2 : list ident) :=
+  match mp1, mp2 with
+  | [], _ | _, [] => ([], mp1, mp2)
+  | i1 :: mp1, i2 :: mp2
+    => if i1 == i2
+       then let '(common, mp1, mp2) := split_common_prefix_ls mp1 mp2 in
+            (i1 :: common, mp1, mp2)
+       else ([], mp1, mp2)
+  end.
+Definition common_prefix_ls (mp1 mp2 : list ident) :=
+  let '(common, _, _) := split_common_prefix_ls mp1 mp2 in common.
+Fixpoint split_modpath (mp : modpath) : (list ident * (dirpath * option (ident * nat)))
+  := match mp with
+     | MPfile f => ([], (f, None))
+     | MPbound f i idx => ([], (f, Some (i, idx)))
+     | MPdot mp i => let '(l, d) := split_modpath mp in (i :: l, d)
+     end.
+(* returns None if either [mp] shares no prefix with [mp] or either modpath is bound, otherwise returns the list of idents of the common prefix *)
+Definition split_common_prefix (mp1 mp2 : modpath) : option ((dirpath * option (ident * nat)) * (list ident * list ident * list ident))
+  := match split_modpath mp1, split_modpath mp2 with
+     | (mp1, f1), (mp2, f2)
+       => if f1 == f2
+          then Some (f1, split_common_prefix_ls (rev mp1) (rev mp2))
+          else None
+     end.
+Definition common_prefix (mp1 mp2 : modpath) : option ((dirpath * option (ident * nat)) * list ident)
+  := option_map (fun '(f, (common, _, _)) => (f, common)) (split_common_prefix mp1 mp2).
+(* Kludge for not having https://github.com/MetaCoq/metacoq/issues/839 *)
+Definition modpath_is_okay (cur_modpath : modpath) (mp : modpath) : bool
+  := andb (modpath_is_absolute mp)
+       match mp with
+       | MPfile _ => true
+       | MPbound _ _ _ => false
+       | MPdot _ _
+         => match common_prefix cur_modpath mp with
+            | None => true (* it's not part of the current module, so it's fine *)
+            | Some (_, []) => true (* only share the top-level, so it can't be a functor *)
+            | Some _ => false
+            end
+       end.
+Definition kername_is_okay (cur_modpath : modpath) (kn : kername) : bool
+  := modpath_is_okay cur_modpath (fst kn).
+
+Definition b_of_dec {P} (H : {P} + {~P}) : bool := if H then true else false.
+Definition bp_of_dec {P H} : @b_of_dec P H = true -> P.
+Proof. cbv [b_of_dec]; destruct H; auto; discriminate. Defined.
+Definition pb_of_dec {P:Prop} {H} : P -> @b_of_dec P H = true.
+Proof. cbv [b_of_dec]; destruct H; auto; discriminate. Defined.
+Definition neg_bp_of_dec {P H} : @b_of_dec P H = false -> ~P.
+Proof. cbv [b_of_dec]; destruct H; auto; discriminate. Defined.
+Definition neg_pb_of_dec {P:Prop} {H} : ~P -> @b_of_dec P H = false.
+Proof. cbv [b_of_dec]; destruct H; tauto. Defined.
+
+(* TODO: move? *)
+Definition kername_of_global_reference (g : global_reference) : option kername
+  := match g with
+     | VarRef _ => None
+     | ConstRef x => Some x
+     | IndRef ind
+     | ConstructRef ind _
+       => Some ind.(inductive_mind)
+     end.
+
+Definition replace_inductive_kn (t : inductive) (ind : inductive) : inductive
+  := {| inductive_mind := ind.(inductive_mind) ; inductive_ind := t.(inductive_ind) |}.
+
+Definition replace_inductive_modpath (mp : modpath) (ind : inductive) : inductive
+  := {| inductive_mind := (mp, snd ind.(inductive_mind)) ; inductive_ind := ind.(inductive_ind) |}.
+
+Definition rebase_global_reference (mp : modpath) (g : global_reference) : global_reference
+  := match g with
+     | VarRef x => VarRef x
+     | ConstRef (_, i) => ConstRef (mp, i)
+     | IndRef ind => IndRef (replace_inductive_modpath mp ind)
+     | ConstructRef ind idx => ConstructRef (replace_inductive_modpath mp ind) idx
+     end.
+
+(* hack around https://github.com/MetaCoq/metacoq/issues/850 *)
+Fixpoint dedup_grefs' (g : list global_reference) (seen : KernameSet.t) : list global_reference
+  := match g with
+     | nil => nil
+     | g :: gs
+       => match kername_of_global_reference g with
+          | None => g :: dedup_grefs' gs seen
+          | Some kn
+            => if KernameSet.mem kn seen
+               then dedup_grefs' gs seen
+               else g :: dedup_grefs' gs (KernameSet.add kn seen)
+          end
+     end.
+Definition dedup_grefs (g : list global_reference) : list global_reference
+  := dedup_grefs' g KernameSet.empty.
+
+Module WithTemplate.
+  Import MetaCoq.Template.Loader.
+  Import MetaCoq.Template.Ast.
+  Import MonadBasicAst MonadAst.
+  Import MetaCoq.Template.TemplateMonad.Common.
+  Import MetaCoq.Template.TemplateMonad.Core.
+
+  (* versions that can be the same for both template and PCUIC, bypassing translation, for performance *)
+  Polymorphic Definition tmQuoteConstantUniversesAndRelevance@{t u} (kn : kername) (bypass_opacity : bool) : TemplateMonad@{t u} (universes_decl * relevance)
+    := cb <- tmQuoteConstant kn bypass_opacity;;
+       let '{| cst_universes := cst_universes ; cst_relevance := cst_relevance |} := cb in
+       ret (cst_universes, cst_relevance).
+
+  Polymorphic Definition tmQuoteInductiveUniverses@{t u} (kn : kername) : TemplateMonad@{t u} universes_decl
+    := mib <- tmQuoteInductive kn;;
+       let '{| ind_universes := ind_universes |} := mib in
+       ret ind_universes.
+
+  (* unfolding Qed'd definitions for the benefit of quotation *)
+  Polymorphic Definition tmUnfoldQed {A} (v : A) : TemplateMonad A
+    := p <- tmQuote v;;
+       v <- match p return TemplateMonad term with
+            | tConst c u
+              => cb <- tmQuoteConstant c true;;
+                 match cb with
+                 | {| cst_body := Some cb |} => tmReturn (subst_instance_constr u cb)
+                 | {| cst_body := None |} => _ <- tmMsg "tmUnfoldQed: failed to find body for";; _ <- tmPrint v;; tmReturn p
+                 end
+            | _ => _ <- tmMsg "tmUnfoldQed: not const";; _ <- tmPrint v;; tmReturn p
+            end;;
+       tmUnquoteTyped A v.
+  Notation transparentify v := (match tmUnfoldQed v return _ with v' => ltac:(run_template_program v' (fun v' => exact v')) end) (only parsing).
+
+
+  Polymorphic Definition tmQuoteToGlobalReference {A} (n : A) : TemplateMonad global_reference
+    := qn <- tmQuote n;;
+       match qn with
+       | tVar id => tmReturn (VarRef id)
+       | tConst c u => tmReturn (ConstRef c)
+       | tInd ind u => tmReturn (IndRef ind)
+       | tConstruct ind idx u => tmReturn (ConstructRef ind idx)
+       | _ => _ <- tmMsg "tmQuoteToGlobalReference: Not a global reference";;
+              _ <- tmPrint n;;
+              _ <- tmPrint qn;;
+              tmFail "tmQuoteToGlobalReference: Not a global reference"
+       end.
+
+  Polymorphic Definition tmObj_magic@{a b t u} {A : Type@{a}} {B : Type@{b}} (x : A) : TemplateMonad@{t u} B
+    := qx <- tmQuote x;;
+       tmUnquoteTyped B qx.
+
+  Polymorphic Definition tmRetype@{a t u} {A : Type@{a}} (x : A) : TemplateMonad@{t u} A
+    := tmObj_magic x.
+
+  Polymorphic Definition tmExtractBaseModPathFromMod (mp : qualid) : TemplateMonad modpath
+    := vs <- tmQuoteModule mp;;
+       match option_map kername_of_global_reference (hd_error vs) with
+       | Some (Some (mp, _)) => ret mp
+       | _ => tmFail "tmExtractBaseModPathFromMod: module has no accessible constant with a kername"
+       end.
+
+  Section with_monad.
+    Context {M} {M_monad : Monad M} (in_domain : bool) (U : Universe.t -> M term).
+
+    #[local]
+      Fixpoint tmRelaxSortsM (t : term) {struct t} : M term
+      := let tmRelaxSortsM_dom t := if in_domain then tmRelaxSortsM t else ret t in
+         match t with
+         | tRel _
+         | tVar _
+         | tInt _
+         | tFloat _
+         | tConst _ _
+         | tInd _ _
+         | tConstruct _ _ _
+           => ret t
+         | tEvar ev args
+           => args <- monad_map tmRelaxSortsM_dom args;;
+              ret (tEvar ev args)
+         | tCast t kind v
+           => t <- tmRelaxSortsM t;;
+              v <- tmRelaxSortsM v;;
+              ret (tCast t kind v)
+         | tProd na ty body
+           => ty <- tmRelaxSortsM_dom ty;;
+              body <- tmRelaxSortsM body;;
+              ret (tProd na ty body)
+         | tLambda na ty body
+           => ty <- tmRelaxSortsM_dom ty;;
+              body <- tmRelaxSortsM body;;
+              ret (tLambda na ty body)
+         | tLetIn na def def_ty body
+           => def <- tmRelaxSortsM_dom def;;
+              def_ty <- tmRelaxSortsM_dom def_ty;;
+              body <- tmRelaxSortsM body;;
+              ret (tLetIn na def def_ty body)
+         | tApp f args
+           => f <- tmRelaxSortsM_dom f;;
+              args <- monad_map tmRelaxSortsM_dom args;;
+              ret (tApp f args)
+         | tCase ci type_info discr branches
+           => type_info <- monad_map_predicate (fun x => ret x) tmRelaxSortsM tmRelaxSortsM type_info;;
+              discr <- tmRelaxSortsM_dom discr;;
+              branches <- monad_map_branches tmRelaxSortsM branches;;
+              ret (tCase ci type_info discr branches)
+         | tProj proj t
+           => t <- tmRelaxSortsM_dom t;;
+              ret (tProj proj t)
+         | tFix mfix idx
+           => mfix <- monad_map (monad_map_def tmRelaxSortsM tmRelaxSortsM) mfix;;
+              ret (tFix mfix idx)
+         | tCoFix mfix idx
+           => mfix <- monad_map (monad_map_def tmRelaxSortsM tmRelaxSortsM) mfix;;
+              ret (tCoFix mfix idx)
+         | tSort s => U s
+         end.
+  End with_monad.
+
+  #[local] Definition is_set (s : Universe.t) : bool
+    := match option_map Level.is_set (Universe.get_is_level s) with
+       | Some true => true
+       | _ => false
+       end.
+
+  #[local] Definition is_type (s : Universe.t) : bool
+    := match Universe.get_is_level s with
+       | Some _ => true
+       | _ => false
+       end.
+
+  #[local] Definition is_only_type (s : Universe.t) : bool
+    := match option_map Level.is_set (Universe.get_is_level s) with
+       | Some false => true
+       | _ => false
+       end.
+
+  Definition tmRelaxSet (in_domain : bool) (prefix : string) (t : term) : term
+    := tmRelaxSortsM
+         (M:=fun T => T) in_domain
+         (fun u => tSort (if is_set u then Universe.of_levels (inr (Level.level (prefix ++ "._Set.0")%bs)) else u))
+         t.
+
+  Module Import PrefixUniverse.
+    Module Level.
+      Definition prefix_with (prefix : string) (l : Level.t) : Level.t
+        := match l with
+           | Level.lzero | Level.lvar _ => l
+           | Level.level u => Level.level (prefix ++ "." ++ u)%bs
+           end.
+    End Level.
+
+    Module LevelExprSet.
+      Module Raw.
+        Definition prefix_with (prefix : string) (l : LevelExprSet.Raw.t) : LevelExprSet.Raw.t
+          := List.map (fun '(l, n) => (Level.prefix_with prefix l, n)) l.
+      End Raw.
+      Lemma prefix_with_Ok {prefix : string} {l : LevelExprSet.Raw.t} (pf : LevelExprSet.Raw.Ok l) : LevelExprSet.Raw.Ok (Raw.prefix_with prefix l).
+      Proof.
+        hnf in *; cbv [Raw.prefix_with] in *; cbn in *.
+        induction l as [|[l n] ls IH]; cbn in *; [ reflexivity | ].
+        apply Bool.andb_true_iff in pf; destruct pf as [pf1 pf2].
+        rewrite IH, Bool.andb_true_r by assumption.
+        clear IH pf2.
+        destruct ls as [|[l' n'] ls]; cbn in *; [ reflexivity | ].
+        destruct l, l'; cbn in *; try assumption.
+        induction prefix as [|?? IH];
+          cbn in *; try assumption.
+        rewrite ByteCompareSpec.compare_eq_refl; assumption.
+      Qed.
+      Definition prefix_with (prefix : string) (l : LevelExprSet.t) : LevelExprSet.t
+        := @LevelExprSet.Mkt (Raw.prefix_with prefix (@LevelExprSet.this l)) (prefix_with_Ok (@LevelExprSet.is_ok l)).
+      Lemma is_empty_prefix_with {prefix} {l} : LevelExprSet.is_empty (prefix_with prefix l) = LevelExprSet.is_empty l.
+      Proof.
+        destruct l as [l pf]; cbn.
+        cbv [LevelExprSet.is_empty prefix_with LevelExprSet.Raw.is_empty]; cbn.
+        destruct l; cbn; reflexivity.
+      Qed.
+    End LevelExprSet.
+
+    Module nonEmptyLevelExprSet.
+      Definition prefix_with (prefix : string) (l : nonEmptyLevelExprSet) : nonEmptyLevelExprSet
+        := {| t_set := LevelExprSet.prefix_with prefix l.(t_set)
+           ; t_ne := eq_trans LevelExprSet.is_empty_prefix_with l.(t_ne) |}.
+    End nonEmptyLevelExprSet.
+
+    Module LevelAlgExpr := nonEmptyLevelExprSet.
+
+    Module Universe.
+      Definition prefix_with (prefix : string) (u : Universe.t) : Universe.t
+        := match u with
+           | Universe.lProp | Universe.lSProp => u
+           | Universe.lType u => Universe.lType (LevelAlgExpr.prefix_with prefix u)
+           end.
+    End Universe.
+  End PrefixUniverse.
+
+  Definition tmRelaxOnlyType (in_domain : bool) (prefix : string) (t : term) : term
+    := tmRelaxSortsM
+         (M:=fun T => T) in_domain
+         (fun u => tSort (PrefixUniverse.Universe.prefix_with prefix u))
+         t.
+
+  Polymorphic Definition tmRetypeMagicRelaxSetInCodomain@{a b t u} (prefix : string) {A : Type@{a}} (B : Type@{b}) (x : A) : TemplateMonad@{t u} B
+    := qx <- tmQuote x;;
+       let qx := tmRelaxSet false prefix qx in
+       tmUnquoteTyped B qx.
+  Polymorphic Definition tmRetypeRelaxSetInCodomain@{a t u} (prefix : string) {A : Type@{a}} (x : A) : TemplateMonad@{t u} A
+    := tmRetypeMagicRelaxSetInCodomain@{a a t u} prefix A x.
+
+  Polymorphic Definition tmRetypeMagicRelaxOnlyType@{a b t u} (prefix : string) {A : Type@{a}} (B : Type@{b}) (x : A) : TemplateMonad@{t u} B
+    := qx <- tmQuote x;;
+       let qx := tmRelaxOnlyType true prefix qx in
+       tmUnquoteTyped B qx.
+  Polymorphic Definition tmRetypeRelaxOnlyType@{a t u} (prefix : string) {A : Type@{a}} (x : A) : TemplateMonad@{t u} A
+    := tmRetypeMagicRelaxOnlyType@{a a t u} prefix A x.
+
+  (* Hack around https://github.com/MetaCoq/metacoq/issues/853 *)
+  Definition tmRetypeAroundMetaCoqBug853 (prefix : string) (t : typed_term) : TemplateMonad typed_term
+    := let '{| my_projT1 := ty ; my_projT2 := v |} := t in
+       ty <- tmRetypeRelaxOnlyType prefix ty;;
+       v <- tmRetypeMagicRelaxOnlyType prefix ty v;;
+       ret {| my_projT1 := ty ; my_projT2 := v |}.
+End WithTemplate.
+Export WithTemplate (transparentify, tmQuoteToGlobalReference, tmRetypeRelaxSetInCodomain, tmRetypeRelaxOnlyType, tmRetypeMagicRelaxSetInCodomain, tmRetypeMagicRelaxOnlyType, tmObj_magic, tmRetype, tmExtractBaseModPathFromMod, tmRetypeAroundMetaCoqBug853, tmQuoteConstantUniversesAndRelevance, tmQuoteInductiveUniverses).
+
+From MetaCoq.Utils Require Export bytestring.
+From MetaCoq.Utils Require Import utils MCList.
+From MetaCoq.Common Require Import MonadBasicAst.
+From MetaCoq.PCUIC Require Import PCUICAst PCUICMonadAst.
+From MetaCoq.TemplatePCUIC Require Import PCUICTemplateMonad Loader.
+
+Require Import Equations.Prop.Classes.
+Require Import Coq.Lists.List.
+
+Export TemplateMonad.Common (export, local, global).
+Import ListNotations.
+
+Local Set Primitive Projections.
+Local Unset Universe Minimization ToSet.
+Local Open Scope bs.
+Import MCMonadNotation.
+
+Class quotation_of {T} (t : T) := quoted_term_of : PCUICAst.term.
+Class ground_quotable T := quote_ground : forall t : T, quotation_of t.
+Class inductive_quotation_of {T} (t : T)
+  := { qinductive : inductive
+     ; qinst : Instance.t
+     ; qquotation : quotation_of t := tInd qinductive qinst }.
+#[local] Instance do_eval_pcuic_quotation : eval_pcuic_quotation := Some cbv.
+Definition default_inductive_quotation_of {T} {t : T} (qt : quotation_of t) (pf : cls_is_true match qt with tInd _ _ => true | _ => false end)
+  : inductive_quotation_of t
+  := match qt return cls_is_true match qt with tInd _ _ => true | _ => false end -> _ with
+     | tInd ind u => fun _ => @Build_inductive_quotation_of T t ind u
+     | _ => fun pf : false = true => match diff_false_true pf with end
+     end pf.
+
+(* returns false iff a term is suitable for quotation at the top-level, i.e., returns true iff it mentions functor-bound arguments or is a local variable or evar *)
+Definition head_term_is_bound (cur_modpath : modpath) (t : term) : bool
+  := match t with
+     | tConst kn _
+     | tInd {| inductive_mind := kn |} _
+     | tConstruct {| inductive_mind := kn |} _ _
+     | tProj {| proj_ind := {| inductive_mind := kn |} |} _
+     | tCase {| ci_ind := {| inductive_mind := kn |} |} _ _ _
+       => negb (kername_is_okay cur_modpath kn)
+     | tVar _
+     | tEvar _ _
+       => true
+     | _ => false
+     end.
+
+Fixpoint head (t : term) : term
+  := match t with
+     | tApp t _
+       => head t
+     | _ => t
+     end.
+
+Polymorphic Definition infer_replacement_inductive {debug : debug_opt} (qt : term) : TemplateMonad (option inductive).
+Proof.
+  simple
+    refine (match qt with
+            | tInd ind u
+            | tConstruct ind _ u
+            | tCase {| ci_ind := ind |} {| puinst := u |} _ _
+              => (indv <- tmUnquote (tInd ind u);;
+                  let '(existT_typed_term _ indv) := indv in
+                  v <- (tmInferInstance None (inductive_quotation_of indv));;
+                  match v with
+                  | my_Some v => ret (Some (replace_inductive_kn ind v.(qinductive)))
+                  | my_None => (if debug then tmPrint (inductive_quotation_of indv) else ret tt);; ret None
+                  end)
+            | tProj {| proj_ind := ind |} t
+              => (t <- tmUnquote t;;
+                  let '(existT_typed_term ty _) := t in
+                  ty <- tmEval hnf ty;;
+                  ty <- tmQuote ty;;
+                  let indv := head ty in
+                  indv <- tmUnquote indv;;
+                  let '(existT_typed_term _ indv) := indv in
+                  v <- (tmInferInstance None (inductive_quotation_of indv));;
+                  match v with
+                  | my_Some v => ret (Some (replace_inductive_kn ind v.(qinductive)))
+                  | my_None => (if debug then tmPrint (qt, inductive_quotation_of ind) else ret tt);; ret None
+                  end)
+            | _ => ret None
+            end).
+Defined.
+
+Polymorphic Fixpoint replace_quotation_of' {debug : debug_opt} (do_top_inference : bool) (qt : term) : TemplateMonad term.
+Proof.
+  specialize (replace_quotation_of' debug).
+  simple
+    refine
+    (let replace_quotation_of' := replace_quotation_of' true in
+     let tmTryInferQuotation t
+       := (t <- tmUnquote t;;
+           let '(existT_typed_term _ t) := t in
+           v <- tmInferInstance None (quotation_of t);;
+           match v return TemplateMonad (option_instance PCUICAst.term) with
+           | my_Some v => ret (@my_Some _ v)
+           | my_None => (if debug then tmPrint (quotation_of t) else ret tt);; ret (@my_None _)
+           end) in
+     let tmInferQuotation t
+       := (v <- tmTryInferQuotation t;;
+           match v return TemplateMonad PCUICAst.term with
+           | my_Some v => ret v
+           | my_None => tmFail "No typeclass instance"
+           end) in
+     let tmMaybeInferQuotation 'tt :=
+       if do_top_inference then tmInferQuotation qt else tmFail "Avoiding loops" in
+     cur_modpath <- tmCurrentModPath tt;;
+     match qt return TemplateMonad PCUICAst.term with
+     | tRel _
+     | tSort _
+     | tPrim _
+     | tConst _ _
+       => if head_term_is_bound cur_modpath qt
+          then tmMaybeInferQuotation tt
+          else ret qt
+     | tConstruct ind idx u
+       => if head_term_is_bound cur_modpath qt
+          then (ind <- infer_replacement_inductive qt;;
+                match ind with
+                | Some ind => ret (tConstruct ind idx u)
+                | None => tmMaybeInferQuotation tt
+                end)
+          else ret qt
+     | tInd ind u
+       => if head_term_is_bound cur_modpath qt
+          then if do_top_inference
+               then (ind <- infer_replacement_inductive qt;;
+                     match ind with
+                     | Some ind => ret (tInd ind u)
+                     | None => tmMaybeInferQuotation tt
+                     end)
+               else tmFail "Avoiding ind loops"
+          else ret qt
+     | tVar _
+       => tmMaybeInferQuotation tt
+     | tEvar ev args => args <- monad_map replace_quotation_of' args;; ret (tEvar ev args)
+     | tLambda na T M => T <- replace_quotation_of' T;; M <- replace_quotation_of' M;; ret (tLambda na T M)
+     | tApp u v => u <- replace_quotation_of' u;; v <- replace_quotation_of' v;; ret (tApp u v)
+     | tProd na A B => A <- replace_quotation_of' A;; B <- replace_quotation_of' B;; ret (tProd na A B)
+     | tLetIn na b ty b' => b <- replace_quotation_of' b;; ty <- replace_quotation_of' ty;; b' <- replace_quotation_of' b';; ret (tLetIn na b ty b')
+     | tProj p c
+       => res <- (if head_term_is_bound cur_modpath qt
+                  then (ind <- infer_replacement_inductive qt;;
+                        match ind with
+                        | Some ind
+                          => let p := {| proj_ind := ind ; proj_npars := p.(proj_npars) ; proj_arg := p.(proj_arg) |} in
+                             ret (inr p)
+                        | None
+                          => res <- tmMaybeInferQuotation tt;;
+                             ret (inl res)
+                        end)
+                  else ret (inr p));;
+          match res with
+          | inl res => ret res
+          | inr p => c <- replace_quotation_of' c;;
+                     ret (tProj p c)
+          end
+     | tFix mfix idx =>
+         mfix' <- monad_map (monad_map_def replace_quotation_of' replace_quotation_of') mfix;;
+         ret (tFix mfix' idx)
+     | tCoFix mfix idx =>
+         mfix' <- monad_map (monad_map_def replace_quotation_of' replace_quotation_of') mfix;;
+         ret (tCoFix mfix' idx)
+     | tCase ci p c brs
+       => res <- (if head_term_is_bound cur_modpath qt
+                  then (ind <- infer_replacement_inductive qt;;
+                        match ind with
+                        | Some ind
+                          => ret (inr {| ci_ind := ind ; ci_npar := ci.(ci_npar) ; ci_relevance := ci.(ci_relevance) |})
+                        | None
+                          => res <- tmMaybeInferQuotation tt;;
+                             ret (inl res)
+                        end)
+                  else ret (inr ci));;
+          match res with
+          | inl res => ret res
+          | inr ci
+            => p' <- monad_map_predicate ret replace_quotation_of' replace_quotation_of' (monad_map_context replace_quotation_of') p;;
+               brs' <- monad_map_branches replace_quotation_of' (monad_map_context replace_quotation_of') brs;;
+               c <- replace_quotation_of' c;;
+               ret (tCase ci p' c brs')
+          end
+     end);
+    try exact _.
+Defined.
+
+Polymorphic Definition replace_quotation_of {debug : debug_opt} {T} (t : T) : TemplateMonad term
+  := qt <- tmQuote t;;
+     replace_quotation_of' false qt.
+
+(** for fancier goals when we have [ground_quotable] for some subterms but not for subterms of those subterms *)
+Polymorphic Definition make_quotation_of {debug : debug_opt} {T} (t : T) : TemplateMonad (quotation_of t).
+Proof.
+  simple
+    refine
+    (qt <- tmQuote t;;
+     let tmInferQuotation t
+       := (t <- tmUnquote t;;
+           let '(existT_typed_term _ t) := t in
+           v <- tmInferInstance None (quotation_of t);;
+           match v with
+           | my_Some v => ret v
+           | my_None => (if debug then tmPrint (quotation_of t) else ret tt);; tmFail "No typeclass instance"
+           end) in
+     cur_modpath <- tmCurrentModPath tt;;
+     if head_term_is_bound cur_modpath qt
+     then ((if debug then tmPrint qt else ret tt);; tmFail "bound argument is not ground")
+     else
+       match qt return TemplateMonad PCUICAst.term with
+       | tSort _
+       | tConst _ _
+       | tConstruct _ _ _
+       | tPrim _
+       | tInd _ _
+         => ret qt
+       | tApp f x
+         => qf <- tmInferQuotation f;;
+            qx <- tmInferQuotation x;;
+            ret (tApp qf qx)
+       | tProj proj t => tmFail "Proj is not reduced"
+       | tRel n => tmFail "Rel is not ground"
+       | tVar id => tmFail "Var is not ground"
+       | tEvar ev args => tmFail "Evar is not ground"
+       | tProd na ty body => tmFail "Prod not yet handled"
+       | tLambda na ty body => tmFail "Lambda not yet handled"
+       | tLetIn na def def_ty body => tmFail "LetIn not yet handled"
+       | tCase ci type_info discr branches => tmFail "Case not yet handled"
+       | tFix mfix idx => tmFail "Fix not yet handled"
+       | tCoFix mfix idx => tmFail "CoFix not yet handled"
+       end);
+    exact _.
+Defined.
+
+Ltac replace_quotation_of_goal _ :=
+  let t := match goal with |- quotation_of ?t => t end in
+  let T := match goal with |- @quotation_of ?T ?t => T end in
+  run_template_program (@replace_quotation_of _ T t) (fun v => exact v).
+
+Ltac make_quotation_of_goal _ :=
+  let t := match goal with |- quotation_of ?t => t end in
+  let T := match goal with |- @quotation_of ?T ?t => T end in
+  run_template_program (@make_quotation_of _ T t) (fun v => exact v).
+
+Ltac adjust_quotation_of_by_econstructor_then tac1 tac2 :=
+  let f := match goal with |- ?f _ => f end in
+  unshelve (let g := open_constr:(f _) in
+            change g);
+  [ unshelve econstructor
+  | ];
+  [ ..
+  | repeat match goal with |- context[?ev] => is_evar ev; generalize ev; intro end ];
+  [ tac1 () ..
+  | tac2 () ].
+
+Ltac adjust_ground_quotable_by_econstructor_inversion _ :=
+  let pf := fresh "pf" in
+  intro pf;
+  adjust_quotation_of_by_econstructor_then ltac:(fun _ => inversion pf; try assumption) ltac:(fun _ => try exact _).
+
+Ltac revert_quotable_hyp _ :=
+  match goal with
+  | [ H : _ |- quotation_of ?v ]
+    => lazymatch v with
+       | H => fail
+       | context[H] => idtac
+       end;
+       revert H;
+       lazymatch goal with
+       | [ |- forall x : ?A, quotation_of (@?P x) ]
+         => assert (quotation_of P);
+            [
+            | intro H;
+              pose proof (_ : quotation_of H);
+              change (quotation_of (P H)); exact _ ]
+       end
+  end.
+Ltac revert_quotable_hyps _ :=
+  repeat revert_quotable_hyp ().
+
+Create HintDb quotation discriminated.
+
+Module Export Instances.
+  (* some performance settings *)
+  #[export] Set Typeclasses Unique Instances.
+  #[export] Instance default_debug : debug_opt | 1000 := false.
+  #[export] Existing Instance do_eval_pcuic_quotation.
+  #[export] Existing Instance quote_ground.
+  #[export] Typeclasses Opaque quotation_of.
+  #[export] Hint Constants Opaque : typeclass_instances.
+  #[export] Typeclasses Transparent Relation_Definitions.relation. (* for setoid_rewrite *)
+  #[export] Hint Extern 0 => progress intros : typeclass_instances.
+  #[export] Hint Extern 0 (quotation_of _) => progress repeat autounfold with quotation in * : typeclass_instances.
+  #[export] Hint Extern 0 (ground_quotable _) => progress repeat autounfold with quotation in * : typeclass_instances.
+  #[export]
+   Hint Extern 0 (quotation_of match ?t with _ => _ end) => is_var t; destruct t : typeclass_instances.
+  #[export]
+   Hint Extern 0 (ground_quotable match ?t with _ => _ end) => is_var t; destruct t : typeclass_instances.
+  #[export]
+   Hint Extern 1 (quotation_of _) => replace_quotation_of_goal () : typeclass_instances.
+  #[export]
+   Hint Extern 2 (quotation_of _) => make_quotation_of_goal () : typeclass_instances.
+  (*#[export]
+   Hint Extern 100 (quotation_of _) => progress revert_quotable_hyps () : typeclass_instances.*)
+  #[export] Hint Mode cls_is_true + : typeclass_instances.
+  #[export] Existing Instances qquotation | 10.
+  (* Hack around COQBUG(https://github.com/coq/coq/issues/16760) *)
+  #[export] Hint Extern 10 (@inductive_quotation_of ?T ?t) => simple notypeclasses refine (@default_inductive_quotation_of T t _ _) : typeclass_instances.
+  #[export] Hint Extern 10 (cls_is_true ?b)
+  => tryif is_evar b then refine (eq_refl true) else tryif has_evar b then fail else vm_compute; reflexivity
+       : typeclass_instances.
+  #[export] Hint Cut [
+      ( _ * )
+        qquotation
+        ( _ * )
+        qquotation
+    ] : typeclass_instances.
+End Instances.
+
+Module PolymorphicInstances.
+  #[export] Polymorphic Instance quote_relax_universe@{a b c} {A : Type@{a}} {q : @quotation_of Type@{b} A} : @quotation_of Type@{c} A | 100 := (q : PCUICAst.term).
+  #[export] Hint Cut [
+      ( _ * )
+        quote_relax_universe
+        ( _ * )
+        quote_relax_universe
+    ] : typeclass_instances.
+End PolymorphicInstances.
+
+Module StrongerInstances.
+  #[export]
+   Hint Extern 1 (quotation_of match ?t with _ => _ end) => destruct t : typeclass_instances.
+  #[export]
+   Hint Extern 1 (ground_quotable match ?t with _ => _ end) => destruct t : typeclass_instances.
+End StrongerInstances.
+
+(** Some helper lemmas for defining quotations *)
+Definition ground_quotable_of_bp {b P} (H : b = true -> P) {qH : quotation_of H} (H_for_safety : P -> b = true) : ground_quotable P.
+Proof.
+  intro p.
+  exact (tApp qH (_ : quotation_of (@eq_refl bool true))).
+Defined.
+
+Definition ground_quotable_neg_of_bp {b P} (H : b = false -> ~P) {qH : quotation_of H} (H_for_safety : ~P -> b = false) : ground_quotable (~P).
+Proof.
+  intro p.
+  exact (tApp qH (_ : quotation_of (@eq_refl bool false))).
+Defined.
+
+Definition ground_quotable_of_dec {P} (H : {P} + {~P}) {qP : quotation_of P} {qH : quotation_of H} : ground_quotable P
+  := ground_quotable_of_bp bp_of_dec pb_of_dec.
+Definition ground_quotable_neg_of_dec {P} (H : {P} + {~P}) {qP : quotation_of P} {qH : quotation_of H} : ground_quotable (~P)
+  := ground_quotable_neg_of_bp neg_bp_of_dec neg_pb_of_dec.
+Definition ground_quotable_neq_of_EqDec {A x y} {qA : quotation_of A} {quoteA : ground_quotable A} {H : EqDec A} {qH : quotation_of H} : ground_quotable (x <> y :> A)
+  := ground_quotable_neg_of_dec (H x y).
+#[export] Hint Extern 1 (ground_quotable (?x <> ?y :> ?A)) => simple notypeclasses refine (@ground_quotable_neq_of_EqDec A x y _ _ _ _) : typeclass_instances.
+
+(* avoid universe inconsistencies *)
+#[export] Polymorphic Instance qfst_cps {A B} {qA : quotation_of A} {qB : quotation_of B} : quotation_of (@fst A B) | 0
+  := PCUICAst.mkApps <% @fst %> [qA; qB].
+#[export] Polymorphic Instance qsnd_cps {A B} {qA : quotation_of A} {qB : quotation_of B} : quotation_of (@snd A B) | 0
+  := PCUICAst.mkApps <% @snd %> [qA; qB].
+#[export] Polymorphic Instance qpair_cps {A B} {qA : quotation_of A} {qB : quotation_of B} : quotation_of (@pair A B) | 0
+  := PCUICAst.mkApps <% @pair %> [qA; qB].
+#[export] Polymorphic Instance qprod_cps {A B} {qA : quotation_of A} {qB : quotation_of B} : quotation_of (@prod A B) | 0
+  := PCUICAst.mkApps <% @prod %> [qA; qB].
+#[export] Polymorphic Instance qSome_cps {A} {qA : quotation_of A} : quotation_of (@Some A) | 0
+  := tApp <% @Some %> qA.
+#[export] Polymorphic Instance qNone_cps {A} {qA : quotation_of A} : quotation_of (@None A) | 0
+  := tApp <% @None %> qA.
+#[export] Polymorphic Instance qoption_cps {A} {qA : quotation_of A} : quotation_of (@option A) | 0
+  := tApp <% @option %> qA.
+#[export] Polymorphic Instance qcons_cps {A} {qA : quotation_of A} : quotation_of (@cons A) | 0
+  := tApp <% @cons %> qA.
+#[export] Polymorphic Instance qnil_cps {A} {qA : quotation_of A} : quotation_of (@nil A) | 0
+  := tApp <% @nil %> qA.
+#[export] Polymorphic Instance qlist_cps {A} {qA : quotation_of A} : quotation_of (@list A) | 0
+  := tApp <% @list %> qA.
+
+Polymorphic Definition ground_quotable_of_iffT {A B} {quoteA : ground_quotable A} {qA : quotation_of A} {qB : quotation_of B} (H : A <~> B) {qH : quotation_of H} : ground_quotable B.
+Proof.
+  intro b.
+  change (@quotation_of B (fst H (snd H b))).
+  make_quotation_of_goal ().
+Defined.
+(* Transparent versions *)
+Definition proj1 {A B} (x : A /\ B) : A := ltac:(apply x).
+Definition proj2 {A B} (x : A /\ B) : B := ltac:(apply x).
+Definition ground_quotable_of_iff {A B : Prop} {quoteA : ground_quotable A} {qA : quotation_of A} {qB : quotation_of B} (H : iff A B) {qH : quotation_of H} : ground_quotable B.
+Proof.
+  intro b.
+  change (@quotation_of B (proj1 H (proj2 H b))).
+  try exact _.
+Defined.
+Definition quote_neg_of_iffT {A B} {quoteA : ground_quotable (A -> False)} {qA : quotation_of A} {qB : quotation_of B} (H : A <~> B) {qH : quotation_of H} : ground_quotable (B -> False).
+Proof.
+  intro nb.
+  assert (na : A -> False) by (intro a; apply nb, H, a).
+  change (@quotation_of (B -> False) (fun b => na (snd H b))).
+  exact _.
+Defined.
+Definition quote_neg_of_iff {A B : Prop} {quoteA : ground_quotable (~A)} {qA : quotation_of A} {qB : quotation_of B} (H : iff A B) {qH : quotation_of H} : ground_quotable (~B).
+Proof.
+  intro nb.
+  assert (na : ~A) by (intro a; apply nb, H, a).
+  change (@quotation_of (~B) (fun b => na (proj2 H b))).
+  exact _.
+Defined.
+
+Ltac unfold_quotation_of _ :=
+  lazymatch goal with
+  | [ |- @quotation_of ?A ?t ]
+    => first [ progress cbv delta [t]
+             | change (@quotation_of A (transparentify t)) ]
+  end.
+
+(* for universe adjustment with [tmDeclareQuotationOfModule], [tmMakeQuotationOfModule] *)
+#[export] Unset MetaCoq Strict Unquote Universe Mode.
+(* N.B. We need to kludge around COQBUG(https://github.com/coq/coq/issues/17303) in Kernames :-( *)
+Polymorphic Definition tmMakeQuotationOfConstants_gen@{d t u _T _above_u'} {debug:debug_opt} (work_around_coq_bug_17303 : bool) (include_submodule : list ident -> bool) (include_supermodule : list ident -> list ident -> bool) (existing_instance : option hint_locality) (base : modpath) (cs : list global_reference) (tmDoWithDefinition : ident -> forall A : Type@{d}, A -> TemplateMonad@{t u} A) : TemplateMonad@{t u} unit
+  := let warn_bad_ctx c ctx :=
+       (_ <- tmMsg "tmPrepareMakeQuotationOfModule: cannot handle polymorphism";;
+        _ <- tmPrint c;;
+        _ <- tmPrint ctx;;
+        tmReturn tt) in
+     let tmDebugMsg s := (if debug
+                          then tmMsg s
+                          else tmReturn tt) in
+     let tmDebugPrint {T : Type@{_T}} (v : T)
+       := (if debug
+           then tmPrint v
+           else tmReturn tt) in
+     let on_bad_relevance r :=
+       (_ <- tmDebugMsg "skipping irrelevant constant";;
+        _ <- tmDebugPrint r;;
+        tmReturn tt) in
+     let make_qname '(mp, name)
+       (* ideally we'd replace _ with __ so that there can't be any collision, but the utility functions aren't written and we don't need it in practice *)
+       := option_map
+            (fun n => "q" ++ n)%bs
+            match split_common_prefix base mp with
+            | None => if include_supermodule [] []
+                      then Some name
+                      else None
+            | Some (_, (_common, [], [])) => Some name
+            | Some (_, (_common, [], postfix))
+              => if include_submodule postfix
+                 then Some (String.concat "__DOT__" postfix ++ "__" ++ name)
+                 else None
+            | Some (_, (_common, base_postfix, postfix))
+              => if include_supermodule base_postfix postfix
+                 then Some ("__DOT_DOT__" ++ String.concat "__DOT__" base_postfix ++ "__SLASH__" ++ String.concat "__DOT__" postfix ++ "__" ++ name)
+                 else None
+            end%bs in
+     let tmDebugSkipGR '(mp, name) :=
+       _ <- tmDebugMsg ("tmMakeQuotationOfConstants_gen: skipping excluded constant " ++ name);;
+       _ <- tmDebugPrint (split_common_prefix base mp);;
+       ret tt in
+     let make_definition '(name, tyv)
+       := ((let tmTyv := tmRetypeAroundMetaCoqBug853 name tyv in
+            _ <- tmDebugPrint tmTyv;;
+            '{| my_projT1 := ty ; my_projT2 := v |} <- tmTyv;;
+            tmDef_name <- tmEval cbv (@tmDoWithDefinition (name:string));;
+            let tmn := tmDef_name ty v in
+            _ <- tmDebugPrint tmn;;
+            n <- tmn;;
+            _ <- tmDebugMsg "tmMakeQuotationOfConstants_gen: tmQuoteToGlobalReference";;
+            qn <- tmQuoteToGlobalReference n;;
+            tmReturn qn) : TemplateMonad global_reference) in
+     let make_instance p
+       := (match existing_instance return TemplateMonad unit with
+           | Some locality
+             => let tmEx := tmExistingInstance locality p in
+                _ <- tmDebugPrint tmEx;;
+                tmEx
+           | None => tmReturn tt
+           end) in
+     let cs := dedup_grefs cs in
+     cs <- tmEval cbv cs;;
+     _ <- tmDebugMsg "tmMakeQuotationOfConstants_gen: looking up module constants";;
+     ps <- monad_map@{_ _ Set _above_u'}
+             (fun r
+              => _ <- tmDebugMsg "tmMakeQuotationOfConstants_gen: handling";;
+                 _ <- tmDebugPrint r;;
+                 match r with
+                 | ConstRef cr
+                   => match make_qname cr with
+                      | None => tmDebugSkipGR cr
+                      | Some qname
+                        => '(univs, rel) <- tmQuoteConstantUniversesAndRelevance cr false;;
+                           match rel with
+                           | Irrelevant => on_bad_relevance cr
+                           | Relevant
+                             => inst <- match univs with
+                                        | Monomorphic_ctx => tmReturn ([] : Instance.t)
+                                        | (Polymorphic_ctx (univs, constraints)) as ctx
+                                          => _ <- warn_bad_ctx cr ctx;;
+                                             tmReturn ([] : Instance.t)
+                                        end;;
+                                let c := tConst cr inst in
+                                _ <- tmDebugMsg "tmMakeQuotationOfConstants_gen: tmUnquote";;
+                                '{| my_projT1 := cty ; my_projT2 := cv |} <- tmUnquote c;;
+                                _ <- tmDebugMsg "tmMakeQuotationOfConstants_gen: tmUnquote done";;
+                                def <- make_definition
+                                         (qname, if work_around_coq_bug_17303
+                                                 then {| my_projT1 := term ; my_projT2 := c |}
+                                                 else {| my_projT1 := @quotation_of cty cv ; my_projT2 := c |});;
+                                make_instance def
+                           end
+                      end
+                 | IndRef ind
+                   => let '{| inductive_mind := r |} := ind in
+                      match make_qname r with
+                      | None => tmDebugSkipGR r
+                      | Some qname
+                        => inst <- (univs <- tmQuoteInductiveUniverses r;;
+                                    match univs with
+                                    | Monomorphic_ctx => tmReturn ([] : Instance.t)
+                                    | (Polymorphic_ctx (univs, constraints)) as ctx
+                                      => _ <- warn_bad_ctx r ctx;;
+                                         tmReturn ([] : Instance.t)
+                                    end);;
+                           let c := tInd ind inst in
+                           _ <- tmDebugMsg "tmMakeQuotationOfConstants_gen: tmUnquote";;
+                           '{| my_projT1 := cty ; my_projT2 := cv |} <- tmUnquote c;;
+                           _ <- tmDebugMsg "tmMakeQuotationOfConstants_gen: tmUnquote done";;
+                           let tmcty := tmRetypeRelaxSetInCodomain@{t t u} qname cty in
+                           _ <- tmDebugPrint tmcty;;
+                           cty <- tmcty;;
+                           let tmcv := tmObj_magic (B:=cty) cv in
+                           _ <- tmDebugPrint tmcv;;
+                           cv <- tmcv;;
+                           let ty := @inductive_quotation_of cty cv in
+                           let v : ty := {| qinductive := ind ; qinst := inst |} in
+                           def <- make_definition
+                                    (qname, {| my_projT1 := ty ; my_projT2 := v |});;
+                           make_instance def
+                      end
+                 | ConstructRef _ _ | VarRef _ => tmReturn tt
+                 end)
+             cs;;
+     ret tt.
+
+Definition tmMakeQuotationOfConstants {debug:debug_opt} (include_submodule : list ident -> bool) (include_supermodule : list ident -> list ident -> bool) (existing_instance : option hint_locality) (base : modpath) (cs : list global_reference) : TemplateMonad unit
+  := tmMakeQuotationOfConstants_gen false include_submodule include_supermodule existing_instance base cs (fun name ty body => @tmDefinition name ty body).
+
+Definition tmMakeQuotationOfConstantsWorkAroundCoqBug17303 {debug:debug_opt} (include_submodule : list ident -> bool) (include_supermodule : list ident -> list ident -> bool) (base : modpath) (cs : list global_reference) : TemplateMonad unit
+  := tmMakeQuotationOfConstants_gen true include_submodule include_supermodule None base cs (fun name ty body => @tmDefinition name ty body).
+
+Definition tmDeclareQuotationOfConstants {debug:debug_opt} (include_submodule : list ident -> bool) (include_supermodule : list ident -> list ident -> bool) (existing_instance : option hint_locality) (base : modpath) (cs : list global_reference) : TemplateMonad unit
+  := tmMakeQuotationOfConstants_gen false include_submodule include_supermodule existing_instance base cs (fun name ty _ => @tmAxiom name ty).
+
+Variant submodule_inclusion := only_toplevel | all_submodules_except (_ : list (list ident)) | toplevel_and_submodules (_ : list (list ident)) | everything.
+
+#[local] Typeclasses Transparent ident IdentOT.t.
+Definition is_submodule_of (super : list ident) (sub : list ident) : bool
+  := firstn #|super| sub == super.
+Definition is_supermodule_of (sub : list ident) (super : list ident) : bool
+  := is_submodule_of super sub.
+Definition include_submodule_of_submodule_inclusion (si : submodule_inclusion) : list ident -> bool
+  := match si with
+     | only_toplevel => fun _ => false
+     | all_submodules_except ls => fun i => negb (existsb (is_supermodule_of i) ls)
+     | toplevel_and_submodules ls => fun i => existsb (is_supermodule_of i) ls
+     | everything => fun _ => true
+     end.
+Definition include_supermodule_of_submodule_inclusion (si : submodule_inclusion) : list ident -> list ident -> bool
+  := match si with
+     | everything => fun _ _ => true
+     | _ => fun _ _ => false
+     end.
+
+Definition tmMakeQuotationOfModule {debug:debug_opt} (include_submodule : submodule_inclusion) (existing_instance : option hint_locality) (m : qualid) : TemplateMonad _
+  := cs <- tmQuoteModule m;;
+     base <- tmLocateModule1 m;;
+     let include_supermodule := include_supermodule_of_submodule_inclusion include_submodule in
+     let include_submodule := include_submodule_of_submodule_inclusion include_submodule in
+     tmMakeQuotationOfConstants include_submodule include_supermodule existing_instance base cs.
+Global Arguments tmMakeQuotationOfModule {_%bool} _ _ _%bs.
+
+Definition tmMakeQuotationOfModuleWorkAroundCoqBug17303 {debug:debug_opt} (include_submodule : submodule_inclusion) (m : qualid) : TemplateMonad _
+  := cs <- tmQuoteModule m;;
+     base <- tmLocateModule1 m;;
+     let include_supermodule := include_supermodule_of_submodule_inclusion include_submodule in
+     let include_submodule := include_submodule_of_submodule_inclusion include_submodule in
+     tmMakeQuotationOfConstantsWorkAroundCoqBug17303 include_submodule include_supermodule base cs.
+Global Arguments tmMakeQuotationOfModuleWorkAroundCoqBug17303 {_%bool} _ _%bs.
+
+Definition tmDeclareQuotationOfModule {debug:debug_opt} (include_submodule : submodule_inclusion) (existing_instance : option hint_locality) (m : qualid) : TemplateMonad _
+  := cs <- tmQuoteModule m;;
+     base <- tmLocateModule1 m;;
+     let include_supermodule := include_supermodule_of_submodule_inclusion include_submodule in
+     let include_submodule := include_submodule_of_submodule_inclusion include_submodule in
+     tmDeclareQuotationOfConstants include_submodule include_supermodule existing_instance base cs.
+Global Arguments tmDeclareQuotationOfModule {_%bool} _ _ _%bs.
+
+(*
+Require Import MSetPositive.
+Instance: debug_opt := true.
+MetaCoq Run (tmMakeQuotationOfModule None "Coq.MSets.MSetPositive.PositiveSet"%bs).
+*)
+
+
 From MetaCoq.Utils Require Export bytestring.
 From MetaCoq.Utils Require Import utils MCList.
 From MetaCoq.Common Require Import MonadBasicAst.
@@ -5,12 +950,125 @@ From MetaCoq.PCUIC.utils Require Import PCUICAstUtils.
 From MetaCoq.PCUIC Require Import PCUICMonadAst PCUICAst PCUICTyping PCUICSpine PCUICArities PCUICSubstitution.
 From MetaCoq.PCUIC.Typing Require Import PCUICWeakeningTyp PCUICWeakeningConfigTyp PCUICWeakeningEnvTyp PCUICClosedTyp.
 From MetaCoq.PCUIC.Syntax Require Import PCUICLiftSubst PCUICClosed PCUICInduction PCUICReflect.
+Set Warnings Append "-notation-overridden".
+
 From MetaCoq.TemplatePCUIC Require Import PCUICTemplateMonad Loader.
 From MetaCoq.SafeChecker Require Import PCUICErrors PCUICTypeChecker PCUICSafeChecker PCUICWfEnvImpl PCUICWfEnv.
-From MetaCoq.Quotation Require Export CommonUtils.
-From MetaCoq.Quotation.ToPCUIC Require Export Init.
-From MetaCoq.Quotation.ToPCUIC Require Coq.Init.
-Import (hints) MetaCoq.Quotation.ToPCUIC.Coq.Init.
+
+Require Import Coq.Lists.List.
+
+
+From MetaCoq.Utils Require Export bytestring. (* for display of quoted objects *)
+From MetaCoq.Utils Require Export ReflectEq.
+From MetaCoq.Utils Require Import All_Forall.
+Require Import Equations.Prop.Classes.
+Import ListNotations.
+
+
+#[export] Instance quote_True : ground_quotable True := ltac:(destruct 1; exact _).
+#[export] Instance quote_False : ground_quotable False := ltac:(destruct 1; exact _).
+#[export] Instance quote_byte : ground_quotable Byte.byte := ltac:(destruct 1; exact _).
+#[export] Instance quote_Empty_set : ground_quotable Empty_set := ltac:(destruct 1; exact _).
+#[export] Instance quote_unit : ground_quotable unit := ltac:(destruct 1; exact _).
+#[export] Instance quote_bool : ground_quotable bool := ltac:(destruct 1; exact _).
+
+#[export] Instance quote_eq {A} {qA : quotation_of A} {quoteA : ground_quotable A} {x y : A} : ground_quotable (x = y :> A) := ltac:(intros []; exact _).
+#[export] Instance quote_eq_refl_l {A} {qA : quotation_of A} {x y : A} {qx : quotation_of x} : ground_quotable (x = y :> A) := ltac:(intros []; exact _).
+#[export] Instance quote_eq_refl_r {A} {qA : quotation_of A} {x y : A} {qy : quotation_of y} : ground_quotable (x = y :> A) := ltac:(intro; subst; exact _).
+
+#[export] Typeclasses Opaque not.
+
+#[export] Hint Unfold is_true : quotation.
+#[export] Hint Unfold lt : quotation.
+#[export] Hint Unfold PeanoNat.Nat.lt : quotation.
+
+#[export] Instance quote_eq_true {b} : ground_quotable (eq_true b) := ltac:(destruct 1; exact _).
+#[export] Instance quote_BoolSpec {P Q : Prop} {b} {qP : quotation_of P} {qQ : quotation_of Q} {quoteP : ground_quotable P} {quoteQ : ground_quotable Q} : ground_quotable (BoolSpec P Q b).
+Proof.
+  destruct b; adjust_ground_quotable_by_econstructor_inversion ().
+Defined.
+#[export] Instance quote_nat : ground_quotable nat := ltac:(induction 1; exact _).
+#[export] Polymorphic Instance quote_option {A} {qA : quotation_of A} {quoteA : ground_quotable A} : ground_quotable (option A) := (ltac:(induction 1; exact _)).
+#[export] Polymorphic Instance quote_sum {A B} {qA : quotation_of A} {qB : quotation_of B} {quoteA : ground_quotable A} {quoteB : ground_quotable B} : ground_quotable (sum A B) := (ltac:(induction 1; exact _)).
+#[export] Polymorphic Instance quote_prod {A B} {qA : quotation_of A} {qB : quotation_of B} {quoteA : ground_quotable A} {quoteB : ground_quotable B} : ground_quotable (prod A B) := (ltac:(induction 1; exact _)).
+#[export] Polymorphic Instance quote_list {A} {qA : quotation_of A} {quoteA : ground_quotable A} : ground_quotable (list A) := (ltac:(induction 1; exact _)).
+#[export] Polymorphic Instance quotation_of_list {A ls} {qA : quotation_of A} {qls : @All A quotation_of ls} : quotation_of ls := ltac:(induction qls; exact _).
+#[export] Instance quote_comparison : ground_quotable comparison := ltac:(destruct 1; exact _).
+#[export] Instance quote_CompareSpec {Peq Plt Pgt : Prop} {qPeq : quotation_of Peq} {qPlt : quotation_of Plt} {qPgt : quotation_of Pgt} {quote_Peq : ground_quotable Peq} {quote_Plt : ground_quotable Plt} {quote_Pgt : ground_quotable Pgt} {c} : ground_quotable (CompareSpec Peq Plt Pgt c).
+Proof.
+  destruct c; adjust_ground_quotable_by_econstructor_inversion ().
+Defined.
+#[export] Instance quote_CompareSpecT {Peq Plt Pgt : Prop} {qPeq : quotation_of Peq} {qPlt : quotation_of Plt} {qPgt : quotation_of Pgt} {quote_Peq : ground_quotable Peq} {quote_Plt : ground_quotable Plt} {quote_Pgt : ground_quotable Pgt} {c} : ground_quotable (CompareSpecT Peq Plt Pgt c) := ltac:(destruct 1; exact _).
+(* Work around masking-absolute-name warning *)
+Module Export Init.
+  Module Decimal.
+    #[export] Instance quote_uint : ground_quotable Decimal.uint := ltac:(induction 1; exact _).
+    #[export] Instance quote_neq_uint {x y} : ground_quotable (x <> y :> Decimal.uint) := ground_quotable_neg_of_dec (@Decimal.uint_eq_dec x y).
+  End Decimal.
+  #[export] Existing Instances Decimal.quote_uint Decimal.quote_neq_uint.
+  Module Hexadecimal.
+    #[export] Instance quote_uint : ground_quotable Hexadecimal.uint := ltac:(induction 1; exact _).
+    #[export] Instance quote_neq_uint {x y} : ground_quotable (x <> y :> Hexadecimal.uint) := ground_quotable_neg_of_dec (@Hexadecimal.uint_eq_dec x y).
+  End Hexadecimal.
+  #[export] Existing Instances Hexadecimal.quote_uint Hexadecimal.quote_neq_uint.
+  Module Number.
+    #[export] Instance quote_uint : ground_quotable Number.uint := ltac:(induction 1; exact _).
+    #[export] Instance quote_neq_uint {x y} : ground_quotable (x <> y :> Number.uint) := ground_quotable_neg_of_dec (@Number.uint_eq_dec x y).
+  End Number.
+  #[export] Existing Instances Number.quote_uint Number.quote_neq_uint.
+End Init.
+#[export] Instance quote_and {A B : Prop} {qA : quotation_of A} {qB : quotation_of B} {quoteA : ground_quotable A} {quoteB : ground_quotable B} : ground_quotable (A /\ B) := (ltac:(destruct 1; exact _)).
+
+#[export] Instance quote_le {n m} : ground_quotable (le n m) := ground_quotable_of_dec (Compare_dec.le_dec n m).
+
+#[export] Polymorphic Instance quote_sig {A} {P : A -> Prop} {qA : quotation_of A} {qP : quotation_of P} {quoteA : ground_quotable A} {quoteP : forall x, quotation_of x -> ground_quotable (P x)} : ground_quotable (@sig A P) := (ltac:(induction 1; exact _)).
+#[export] Polymorphic Instance quote_sig2 {A} {P Q : A -> Prop} {qA : quotation_of A} {qP : quotation_of P} {qQ : quotation_of Q} {quoteA : ground_quotable A} {quoteP : forall x, quotation_of x -> ground_quotable (P x)} {quoteQ : forall x, quotation_of x -> ground_quotable (Q x)} : ground_quotable (@sig2 A P Q) := (ltac:(induction 1; exact _)).
+#[export] Polymorphic Instance quote_sigT {A P} {qA : quotation_of A} {qP : quotation_of P} {quoteA : ground_quotable A} {quoteP : forall x, quotation_of x -> ground_quotable (P x)} : ground_quotable (@sigT A P) := (ltac:(induction 1; exact _)).
+#[export] Polymorphic Instance quote_sigT2 {A} {P Q} {qA : quotation_of A} {qP : quotation_of P} {qQ : quotation_of Q} {quoteA : ground_quotable A} {quoteP : forall x, quotation_of x -> ground_quotable (P x)} {quoteQ : forall x, quotation_of x -> ground_quotable (Q x)} : ground_quotable (@sigT2 A P Q) := (ltac:(induction 1; exact _)).
+#[export] Instance quote_sumbool {A B : Prop} {qA : quotation_of A} {qB : quotation_of B} {quoteA : ground_quotable A} {quoteB : ground_quotable B} : ground_quotable (sumbool A B) := ltac:(destruct 1; exact _).
+#[export] Instance quote_sumor {A} {B : Prop} {qA : quotation_of A} {qB : quotation_of B} {quoteA : ground_quotable A} {quoteB : ground_quotable B} : ground_quotable (sumor A B) := ltac:(destruct 1; exact _).
+
+Definition quote_or_dec_l {P Q : Prop} (decP : {P} + {~P}) {qP : quotation_of P} {qQ : quotation_of Q} {quoteP : ground_quotable P} {quoteQ : ground_quotable Q} : ground_quotable (or P Q).
+Proof.
+  destruct decP.
+  all: intro pf; adjust_quotation_of_by_econstructor_then ltac:(fun _ => destruct pf; first [ eassumption | tauto ]) ltac:(fun _ => exact _).
+Defined.
+Definition quote_or_dec_r {P Q : Prop} (decQ : {Q} + {~Q}) {qP : quotation_of P} {qQ : quotation_of Q} {quoteP : ground_quotable P} {quoteQ : ground_quotable Q} : ground_quotable (or P Q).
+Proof.
+  destruct decQ.
+  all: intro pf; adjust_quotation_of_by_econstructor_then ltac:(fun _ => destruct pf; first [ eassumption | tauto ]) ltac:(fun _ => exact _).
+Defined.
+
+(* These are not possible *)
+(*
+#[export] Instance quote_or : ground_quotable or := ltac:(destruct 1; exact _). (A B:Prop) : Prop :=
+#[export] Instance quote_ex : ground_quotable ex := ltac:(destruct 1; exact _). (A:Type) (P:A -> Prop) : Prop :=
+#[export] Instance quote_ex2 : ground_quotable ex2 := ltac:(destruct 1; exact _). (A:Type) (P Q:A -> Prop) : Prop :=
+#[export] Instance quote_inhabited : ground_quotable inhabited := ltac:(destruct 1; exact _). (A:Type) : Prop := inhabits : A -> inhabited A.
+*)
+
+#[export] Instance quote_neq_True {x y : True} : ground_quotable (x <> y).
+Proof. destruct x, y; intro; exfalso; congruence. Defined.
+#[export] Instance quote_neq_False {x y : False} : ground_quotable (x <> y) := ltac:(destruct x).
+#[export] Instance quote_neq_byte {x y} : ground_quotable (x <> y :> Byte.byte) := ground_quotable_neg_of_dec (@Byte.byte_eq_dec x y).
+#[export] Instance quote_neq_Empty_set {x y : Empty_set} : ground_quotable (x <> y) := ltac:(destruct x).
+#[export] Instance quote_neq_unit {x y : unit} : ground_quotable (x <> y).
+Proof. destruct x, y; intro; exfalso; congruence. Defined.
+#[export] Instance quote_neq_bool {x y} : ground_quotable (x <> y :> bool) := ground_quotable_neg_of_dec (@Bool.bool_dec x y).
+#[export] Instance quote_neq_nat {x y} : ground_quotable (x <> y :> nat) := ground_quotable_neg_of_dec (@PeanoNat.Nat.eq_dec x y).
+Scheme Equality for comparison.
+#[export] Instance quote_neq_comparison {x y} : ground_quotable (x <> y :> comparison) := ground_quotable_neg_of_dec (@comparison_eq_dec x y).
+
+#[export] Instance quote_nle {n m} : ground_quotable (~le n m) := ground_quotable_neg_of_dec (Compare_dec.le_dec n m).
+
+Definition option_eq_None_dec_r {A} {l : option A} : {l = None} + {l <> None}.
+Proof. destruct l; [ right | left ]; try reflexivity; congruence. Defined.
+Definition option_eq_None_dec_l {A} {l : option A} : {None = l} + {None <> l}.
+Proof. destruct l; [ right | left ]; try reflexivity; congruence. Defined.
+#[export] Instance quote_option_neq_None_r {A} {qA : quotation_of A} (l : option A) {ql : quotation_of l} : ground_quotable (l <> None)
+  := ground_quotable_neg_of_dec option_eq_None_dec_r.
+#[export] Instance quote_option_neq_None_l {A} {qA : quotation_of A} (l : option A) {ql : quotation_of l} : ground_quotable (None <> l)
+  := ground_quotable_neg_of_dec option_eq_None_dec_l.
 Require Import Equations.Prop.Classes.
 Require Import Coq.Lists.List.
 Export TemplateMonad.Common (export, local, global).
@@ -175,7 +1233,7 @@ Notation typing_restriction_for_globals ls
        (only parsing).
 
 
-Module Export Instances.
+Module Export Instances'.
   #[export] Existing Instance Build_infer_quotation_of_well_typed.
   #[export] Hint Extern 0 (infer_quotation_of_well_typed ?qt)
   => simple notypeclasses refine (@Build_infer_quotation_of_well_typed qt _ _ _ _ _ _);
@@ -188,7 +1246,7 @@ Module Export Instances.
     := {| config.checker_flags_constraint cf := true
        ; config.global_env_ext_constraint Σ := true |}.*)
   #[export] Existing Instance typing_quote_ground.
-End Instances.
+End Instances'.
 
 Definition lift_step
   : forall (lift' : nat -> nat -> term -> term) (n k : nat) (t : term), term.
@@ -1024,704 +2082,3 @@ Proof.
   subst Σ0'.
   intros t wfΣ.
   Time  (intros; lazymatch goal with |- @typing ?cf ?Σ ?Γ ?t ?T => pose proof (@quotation_check_valid config.strictest_checker_flags Σ0 Γ t T) as H' end; clear H'; admit). Timeout 3 Qed.
-  handle_typing_by_factoring ().
-  all: [ > handle_typing_by_tc () .. | ].
-  all: subst Σ.
-  all: [ > handle_typing_tc_side_conditions () .. | ].
-  all: [ > ].
-  repeat match goal with H : _ |- _ => revert H end.
-  match goal with |- ?T => refine (@id T _) end.
-
-
-Finished transaction in 0.161 secs (0.161u,0.s) (successful)
-                              Finished transaction in 0.2 secs (0.2u,0.s) (successful)
-Finished transaction in 0.195 secs (0.195u,0.s) (successful)
-                              Finished transaction in 7.062 secs (7.062u,0.s) (successful)
-Finished transaction in 0.116 secs (0.116u,0.s) (successful)
-
-         pose
-  Time admit. Time Qed.
-Finished transaction in 0.053 secs (0.053u,0.s) (successful)
-                              Finished transaction in 0.17 secs (0.17u,0.s) (successful)
-  Time abstract (intros; handle_typing_by_safechecker config.strictest_checker_flags Σ0).
-  Time Qed.
-  all: todo "foo". Qed.
-
-  todo "foo".
-Qed.
-
-  Search compatible compatibleb.
-  2: apply extends_refl.
-  2: etransitivity
-  Search extends merge_global_envs.
-  2: apply extends_m
-  all: try assumption.
-  all: subst
-  all: lazymatch goal iwth
-  Set Printing Implicit.
-  exact _.
-  end.
-  end.
-  run_template_program p (fun v => pose v as v').
-  Lemma closed_substitution_cps {cf : config.checker_flags} {Σ : global_env_ext}
-  (s : list term)
-  (Γ' : list term)
-  (t T : term)
-  (wfΣ : wf Σ)
-
-
-  closed_substitution_nolift {cf : config.checker_flags} {Σ}
-  (s : list term)
-  (Γ' : list term)
-  (t T : term)
-  (Hs : All2 (fun t T => Σ ;;; [] |- t : T) s Γ')
-  (wfΣ : wf Σ)
-  (Γ'' := List.map (fun ty => {| BasicAst.decl_name := {| binder_name := nAnon; binder_relevance := Relevant |} ; BasicAst.decl_body := None ; BasicAst.decl_type := ty |}) Γ')
-  (Ht : Σ ;;; Γ'' |- t : T)
-  : Σ ;;; [] |- subst_nolift s 0 t : subst_nolift s 0 T.
-Proof.
-  erewrite <- !closed_subst_nolift by eassumption.
-  now eapply @closed_substitution.
-Qed.
-  cbn in p0.
-    => run_template_program (collect_constants t []) (fun v => pose v)
-  end.
-
-  Search typing subst.
-  Set Printing Implicit.
-  Print context_decl.
-  Print BasicAst.context_decl.
-  Print aname.
-  Print binder_annot.
-  Check @substitution.
-  epose (@substitution cf Σ Hwf []
-           [{| BasicAst.decl_name := {| binder_name := nAnon; binder_relevance := Relevant |} ; BasicAst.decl_body := None ; BasicAst.decl_type := ltac:(lazymatch type of qtyH with @quotation_of_well_typed _ _ _ ?T _ => exact T end) |};
-            {| BasicAst.decl_name := {| binder_name := nAnon; binder_relevance := Relevant |} ; BasicAst.decl_body := None ; BasicAst.decl_type := ltac:(lazymatch type of qtyP with @quotation_of_well_typed _ _ _ ?T _ => exact T end) |}] [qH; qP] []
-        (tApp (tRel 0)
-       (tApp
-          (tApp
-             (tConstruct
-                {|
-                  inductive_mind := (MPfile ["Logic"; "Init"; "Coq"], "eq");
-                  inductive_ind := 0
-                |} 0 [])
-             (tInd
-                {|
-                  inductive_mind := (MPfile ["Datatypes"; "Init"; "Coq"], "bool");
-                  inductive_ind := 0
-                |} []))
-          (tConstruct
-             {|
-               inductive_mind := (MPfile ["Datatypes"; "Init"; "Coq"], "bool");
-               inductive_ind := 0
-             |} 0 [])))
-        (tRel 1)
-        ) as v.
-  clearbody v.
-  cbn in v.
-  rewrite !lift_closed in v.
-  cbv [subst_context] in v.
-  cbv [fold_context_k] in v.
-  cbn in v.
-  apply v.
-  { constructor.
-    constructor.
-    constructor.
-    all: rewrite !subst_closedn.
-    3: apply qtyH.
-    1:apply qtyP.
-    all: try assumption.
-    all: try solve [ constructor ].
-    change (closedn 0) with (closedn #|[]:context|).
-    eapply type_closed.
-    eapply qtyH.
-    all: try eassumption.
-    now constructor. }
-    apply closedn_
-            eapply
-    3: { move qtyH at bottom.
-         hnf in qtyH.
-         Unset Printing Implicit.
-    2: apply qtyH.
-    all: cbv [subst0]; cbn.
-    2: {
-  Unset Printing Implicit.
-  Print aname.
-  Check {| binder_name := nAnon; binder_relevance := Relevant |} : aname.
-  Check nAnon.
-  Search closedn lift.
-  Print lift0.
-  all: repeat
-         repeat first [ assumption
-                    | now constructor
-                    | progress cbv [subst1] in *
-                    | rewrite subst_closedn
-                    | progress cbn [List.app ind_type]
-                    | progress cbn [subst_instance subst_instance_constr subst_instance_univ]
-                    | progress cbn [type_of_constructor]
-                    | progress cbv [PCUICLookup.declared_minductive_gen]
-                    | match goal with
-                      | [ |- _;;;_ |- tApp _ _ : _ ] => eapply type_App
-                      | [ |- _;;;_ |- tInd _ _ : _ ] => eapply type_Ind
-                      | [ |- _;;;_ |- tConstruct _ _ _ : _ ] => eapply type_Construct
-                      | [ H : @quotation_of_well_typed _ _ _ _ ?qP  |- _;;;_ |- ?qP : _ ]
-                        => (idtac + eapply type_Cumul); [ eapply H | .. ]
-                      | [ H : @quotation_of_well_typed _ _ _ _ ?qP  |- is_true (closedn 0 ?qP) ]
-                        => eapply @subject_closed with (Γ:=[]); [ | eapply H ]; tea
-                      | [ |- wf_local _ [] ] => constructor
-                      | [ |- wf_local _ (_ ,, _) ] => constructor
-                      | [ |- _;;;_ |- tProd _ _ _ : _ ] => eapply type_Prod
-                      | [ |- _;;;_ |- tSort _ : _ ] => eapply type_Sort
-                      | [ |- lift_typing _ _ _ _ _ ] => hnf; try eexists
-                      | [ |- context[tApp ?f ?x] ]
-                        => change (tApp f x) with (mkApps f [x])
-                      | [ |- context[mkApps (mkApps ?f ?x) ?y] ]
-                        => change (mkApps (mkApps f x) y) with (mkApps f (x ++ y))
-                      | [ |- _;;;_ |- mkApps _ _ : _ ]
-                        => eapply type_mkApps
-                      | [ |- PCUICArities.typing_spine _ _ _ _ _ ]
-                        => econstructor
-                      | [ |- declared_inductive _ _ _ _ ] => eapply declared_inductive_from_gen; constructor; hnf
-                      | [ |- declared_constructor _ _ _ _ _ ] => eapply declared_constructor_from_gen; repeat apply conj
-                      | [ |- isType _ _ (tProd _ _ _) ] => apply isType_tProd; split
-                      | [ |- isType _ _ (tSort _) ] => apply isType_Sort
-                      | [ |- _ = _ ] => eassumption
-                      | [ |- _;;;_ |- tSort _ <=s tSort _ ] => apply cumul_Sort
-                      end ].
-  all: lazymatch goal with
-       | [ |- isType _ _ _ ] => cbn; econstructor
-       | [ |- wf_universe _ _ ] => idtac
-       | _ => cbn
-       end.
-  all: repeat
-         repeat first [ assumption
-                      | reflexivity
-                    | progress cbv [subst1] in *
-                    | rewrite subst_closedn
-                    | progress cbn [List.app ind_type]
-                    | progress cbn [subst_instance subst_instance_constr subst_instance_univ]
-                    | progress cbn [type_of_constructor]
-                    | progress cbv [PCUICLookup.declared_minductive_gen]
-                    | match goal with
-                      | [ |- context[tApp ?f ?x] ]
-                        => change (tApp f x) with (mkApps f [x])
-                      | [ |- context[mkApps (mkApps ?f ?x) ?y] ]
-                        => change (mkApps (mkApps f x) y) with (mkApps f (x ++ y))
-                      | [ |- _;;;_ |- mkApps _ _ : _ ]
-                        => eapply type_mkApps
-                      | [ |- _;;;_ |- tInd _ _ : _ ] => eapply type_Ind
-                      | [ |- _;;;_ |- tConstruct _ _ _ : _ ] => eapply type_Construct
-                      | [ |- _;;;_ |- tRel _ : _ ] => (idtac + eapply type_Cumul); [ eapply type_Rel | .. ]
-                      | [ H : @quotation_of_well_typed _ _ _ _ ?qP  |- _;;;_ |- ?qP : _ ]
-                        => (idtac + eapply type_Cumul); [ eapply H | .. ]
-                      | [ H : @quotation_of_well_typed _ _ _ _ ?qP  |- is_true (closedn 0 ?qP) ]
-                        => eapply @subject_closed with (Γ:=[]); [ | eapply H ]; tea
-                      | [ |- wf_local _ [] ] => constructor
-                      | [ |- wf_local _ (_ ,, _) ] => constructor
-                      | [ |- _;;;_ |- tProd _ _ _ : _ ] => eapply type_Prod
-                      | [ |- _;;;_ |- tSort _ : _ ] => eapply type_Sort
-                      | [ |- lift_typing _ _ _ _ _ ] => hnf; try eexists
-                      | [ |- PCUICArities.typing_spine _ _ _ _ _ ]
-                        => econstructor
-                      | [ |- declared_inductive _ _ _ _ ] => eapply declared_inductive_from_gen; constructor; hnf
-                      | [ |- declared_constructor _ _ _ _ _ ] => eapply declared_constructor_from_gen; repeat apply conj
-                      | [ |- isType _ _ (tProd _ _ _) ] => apply isType_tProd; split
-                      | [ |- isType _ _ (tSort _) ] => apply isType_Sort
-                      | [ |- _ = _ ] => eassumption
-                      | [ |- _;;;_ |- tSort _ <=s tSort _ ] => apply cumul_Sort
-                      end ].
-
-  all: lazymatch goal with
-       | [ |- isType _ _ _ ] => cbn; econstructor
-       | [ |- wf_universe _ _ ] => idtac
-       | _ => cbn
-       end.
-  all: repeat
-         repeat first [ assumption
-                      | reflexivity
-                    | progress cbv [subst1] in *
-                    | rewrite subst_closedn
-                    | progress cbn [List.app ind_type]
-                    | progress cbn [subst_instance subst_instance_constr subst_instance_univ]
-                      | progress cbn [type_of_constructor]
-                      | progress cbn [lift0 decl_type vass]
-                    | progress cbv [PCUICLookup.declared_minductive_gen]
-                    | match goal with
-                      | [ |- context[tApp ?f ?x] ]
-                        => change (tApp f x) with (mkApps f [x])
-                      | [ |- context[mkApps (mkApps ?f ?x) ?y] ]
-                        => change (mkApps (mkApps f x) y) with (mkApps f (x ++ y))
-                      | [ |- _;;;_ |- mkApps _ _ : _ ]
-                        => eapply type_mkApps
-                      | [ |- _;;;_ |- tInd _ _ : _ ] => (idtac + eapply type_Cumul); [ eapply type_Ind | .. ]
-                      | [ |- _;;;_ |- tConstruct _ _ _ : _ ] => eapply type_Construct
-                      | [ |- _;;;_ |- tRel _ : _ ] => (idtac + eapply type_Cumul); [ eapply type_Rel | .. ]
-                      | [ H : @quotation_of_well_typed _ _ _ _ ?qP  |- _;;;_ |- ?qP : _ ]
-                        => (idtac + eapply type_Cumul); [ eapply H | .. ]
-                      | [ H : @quotation_of_well_typed _ _ _ _ ?qP  |- is_true (closedn 0 ?qP) ]
-                        => eapply @subject_closed with (Γ:=[]); [ | eapply H ]; tea
-                      | [ |- wf_local _ [] ] => constructor
-                      | [ |- wf_local _ (_ ,, _) ] => constructor
-                      | [ |- _;;;_ |- tProd _ _ _ : _ ] => eapply type_Prod
-                      | [ |- _;;;_ |- tSort _ : _ ] => eapply type_Sort
-                      | [ |- lift_typing _ _ _ _ _ ] => hnf; try eexists
-                      | [ |- PCUICArities.typing_spine _ _ _ _ _ ]
-                        => econstructor
-                      | [ |- declared_inductive _ _ _ _ ] => eapply declared_inductive_from_gen; constructor; hnf
-                      | [ |- declared_constructor _ _ _ _ _ ] => eapply declared_constructor_from_gen; repeat apply conj
-                      | [ |- isType _ _ (tProd _ _ _) ] => apply isType_tProd; split
-                      | [ |- isType _ _ (tSort _) ] => apply isType_Sort
-                      | [ |- _ = _ ] => eassumption
-                      | [ |- _;;;_ |- tSort _ <=s tSort _ ] => apply cumul_Sort
-                      end ].
-  all: lazymatch goal with
-       | [ |- wf_universe _ _ ] => shelve
-       | _ => idtac
-       end.
-  2: { constructor 1; try refine (@eq_refl bool true).
-       2: { hnf.
-            Print PCUICEquality.eq_term_upto_univ_napp.
-             reflexivity.
-             constructor.
-             reflexivity.
-        cbn.
-       refine (eq_refl true).
-        cbn.
-  2: { match goal with
-  match goal
-  all: match goal with |- _ ;;; _ |- ?e : _ => is_evar e; shelve | _ => idtac end.
-  4: {
-  match goal with
-  all: try apply cumul_Sort.
-  Print cumulSpec0.
-Set Printing All.
-
-  all:
-  21: { cbv [type_of_constructor inductive_mind fst snd cstr_type ind_bodies subst0 inds List.length subst_instance subst_instance_constr].
-  all: lazymatch goal with
-       | [ |- isType _ _ _ ] => econstructor
-       | _ => idtac
-       end.
-    end ].
-  all: cbn.
-  Search isType tApp.
-  47: {
-  all: cbn.
-  53: { cbv [PCUICLookup.declared_minductive_gen].
-  Search isType tRel.
-  cbn -[wf_universe].
-  cbv [subst_instance subst_instance_univ0 NonEmptySetFacts.map].
-  Set Printing All.
-  Search isType tSort.
-  lazymatch goal with
-  end.
-  Search isType tProd.
-  all: repeat first [ progress cbn [type_of_constructor ind_type ind_bodies inductive_ind nth_error]
-                    | eassumption
-                    | reflexivity
-                    | match goal with
-                      | [ |- declared_inductive _ _ _ _ ] => eapply declared_inductive_from_gen; constructor; hnf
-                      | [ |- declared_constructor _ _ _ _ _ ] => eapply declared_constructor_from_gen; repeat apply conj
-                      end ].
-  all: repeat first [ progress cbn [type_of_constructor ind_type ind_bodies inductive_ind nth_error]
-                    | progress cbv [type_of_constructor ind_type]
-                    | eassumption
-                    | reflexivity
-                    | match goal with
-                      | [ |- declared_inductive _ _ _ _ ] => eapply declared_inductive_from_gen; constructor; hnf
-                      | [ |- declared_constructor _ _ _ _ _ ] => eapply declared_constructor_from_gen; repeat apply conj
-                      | [ |- isType _ _ _ ] => eexists
-                      end ].
-  all: cbn.
-  all: repeat first [ reflexivity
-                    | eassumption
-                    | match goal with
-                      | [ |- _;;;_ |- tProd _ _ _ : _ ] => eapply type_Prod
-                      | [ |- _;;;_ |- tSort _ : _ ] => eapply type_Sort
-                      | [ |- _;;;_ |- tRel _ : _ ] => (idtac + eapply type_Cumul); [ eapply type_Rel | .. ]
-                      | [ |- _;;;_ |- tInd _ _ : _ ] => (idtac + eapply type_Cumul); [ eapply type_Ind | .. ]
-                      | [ |- wf_local _ [] ] => constructor
-                      | [ |- wf_local _ [] ] => constructor
-                      | [ |- wf_local _ (_ ,, _) ] => constructor
-                      | [ |- lift_typing _ _ _ _ _ ] => hnf; try eexists
-                      | [ |- declared_inductive _ _ _ _ ] => eapply declared_inductive_from_gen; constructor; hnf
-                      | [ |- declared_constructor _ _ _ _ _ ] => eapply declared_constructor_from_gen; repeat apply conj
-                      end ].
-  all: match goal with |- wf_universe _ _ => shelve | _ => idtac end.
-  all: cbn.
-  cbn.
-  Search wf_universe.
-  2: {  Set Printing All.
-                      | [ |- _;;;_ |- tInd _ _ : _ ] => eapply type_Ind
-                      | [ |- _;;;_ |- tConstruct _ _ _ : _ ] => eapply type_Construct
-Print type_of_constructor.
-  hnf.
-  Print isType.
-  cbn [ind_type].
-  all: lazymatch goal with
-       | _ => idtac
-       end.
-  { constructor.
-    hnf.
-    eassumption.
-  match goal with
-  end.
-  Search declared_inductive lookup_env.
-  Set Printing Implicit.
-  { repeat match goal with
-           end.
-    Search eqb.
-    match goal with
-    end.
-
-  24: {
-  Locate weaken_ctx.
-  Check weaken_ctx.
-  HERE
-  3: { cbn.
-       match goal with
-       end.
-  7: {
-    match goal with
-   end.
-
-  eapply type_Ind.
-  eapply type_mkApps.
-  match goal with
-  end.
-  eapply type_App.
-  2: {
-    match goal with
-    cbn [lift_typing].
-  2: constructor.
-  3: { lazymatch goal with
-    end.
-           (idtac + eapply type_Cumul); [ eapply H | .. ]
-                                         ; eassumption
-
-        constructor 3
-  all: repeat first [ assumption
-                    | match goal with
-                      | [ |- _;;;_ |- tApp _ _ : _ ] => eapply type_App
-                      | [ H : @quotation_of_well_typed _ _ _ _ ?qP  |- _;;;_ |- ?qP : _ ]
-                        => (idtac + eapply type_Cumul); [ eapply H | .. ]
-                      end ].
-  2: {
-  all: repeat first [ assumption
-                    | match goal with
-                      | [ |- _;;;_ |- tApp _ _ : _ ] => eapply type_App
-                      | [ H : @quotation_of_well_typed _ _ _ _ ?qP  |- _;;;_ |- ?qP : _ ]
-                        => (idtac + eapply type_Cumul); [ eapply H | .. ]
-                      end ].
-  2: { match goal with
-                      | [ |- _;;;_ |- tApp _ _ : _ ] => eapply type_App
-                      | [ H : @quotation_of_well_typed _ _ _ _ ?qP  |- _;;;_ |- ?qP : _ ]
-                        => (idtac + eapply type_Cumul); [ eapply H | .. ]
-                      end.
-  eapply type_Prod.
-  3: {
-  all: repeat first [ assumption
-                    | match goal with
-                      | [ |- _;;;_ |- tApp _ _ : _ ] => eapply type_App
-                      | [ |- _;;;_ |- qH : _ ]
-                        => (idtac + eapply type_Cumul); [ eapply qtyH | .. ]
-                      | [ |- _;;;_ |- qP : _ ]
-                        => (idtac + eapply type_Cumul); [ eapply qtyP | .. ]
-                      end ].
-  3: { match goal with
-                 | [ |- _;;;_ |- qP : _ ]
-                   => (idtac + eapply type_Cumul); [ eapply qtyP | .. ]
-    end.
-      eapply qtyP.
-  2: { exactly_once econstructor.
-       Show Proof.
-  2: eapply qtyH.
-         | [ |- _;;;_ |- tProd _ _ _ : _ ] => eapply type_Prod
-  { eapply type_App.
-    eapply type_Prod.
-    3: { eapply qtyH; assumption.
-         assumption.
-         assumption.
-         assumption.
-      hnf in qtyH.
-
-  cbn [mkApps].
-
-  Search typing tApp.
-  Search mkApps typing.
-
-  hnf in qtyH.
-  hnf.
-
-
-Class quotation_of_well_typed {Pcf : config.typing_restriction} {T} (t : T) {qT : quotation_of T} {qt : quotation_of t} := typing_quoted_term_of : forall cf Σ Γ, config.checker_flags_constraint cf -> config.global_env_ext_constraint Σ -> wf_local Σ Γ -> Σ ;;; Γ |- qt : qT.
-Class ground_quotable_well_typed {Pcf : config.typing_restriction} T {qT : quotation_of T} {quoteT : ground_quotable T} := typing_quote_ground : forall t : T, quotation_of_well_typed t.
-
-
-ground_quotable_well_typed {Pcf : config.typing_restriction} T {qT : quotation_of T} {quoteT : ground_quotable T} := typing_quote_ground : forall t : T, quotation_of_well_typed t.
-
-(** Some helper lemmas for defining quotations *)
-Definition ground_quotable_of_bp {b P} (H : b = true -> P) {qH : quotation_of H} (H_for_safety : P -> b = true) : ground_quotable P.
-Proof.
-  intro p.
-  exact (Ast.mkApps qH [_ : quotation_of (@eq_refl bool true)]).
-Defined.
-
-Definition ground_quotable_neg_of_bp {b P} (H : b = false -> ~P) {qH : quotation_of H} (H_for_safety : ~P -> b = false) : ground_quotable (~P).
-Proof.
-  intro p.
-  exact (Ast.mkApps qH [_ : quotation_of (@eq_refl bool false)]).
-Defined.
-
-Definition ground_quotable_of_dec {P} (H : {P} + {~P}) {qP : quotation_of P} {qH : quotation_of H} : ground_quotable P
-  := ground_quotable_of_bp bp_of_dec pb_of_dec.
-Definition ground_quotable_neg_of_dec {P} (H : {P} + {~P}) {qP : quotation_of P} {qH : quotation_of H} : ground_quotable (~P)
-  := ground_quotable_neg_of_bp neg_bp_of_dec neg_pb_of_dec.
-Definition ground_quotable_neq_of_EqDec {A x y} {qA : quotation_of A} {quoteA : ground_quotable A} {H : EqDec A} {qH : quotation_of H} : ground_quotable (x <> y :> A)
-  := ground_quotable_neg_of_dec (H x y).
-#[export] Hint Extern 1 (ground_quotable (?x <> ?y :> ?A)) => simple notypeclasses refine (@ground_quotable_neq_of_EqDec A x y _ _ _ _) : typeclass_instances.
-
-(* avoid universe inconsistencies *)
-#[export] Polymorphic Instance qfst_cps {A B} {qA : quotation_of A} {qB : quotation_of B} : quotation_of (@fst A B) | 0
-  := tApp <% @fst %> [qA; qB].
-#[export] Polymorphic Instance qsnd_cps {A B} {qA : quotation_of A} {qB : quotation_of B} : quotation_of (@snd A B) | 0
-  := tApp <% @snd %> [qA; qB].
-#[export] Polymorphic Instance qpair_cps {A B} {qA : quotation_of A} {qB : quotation_of B} : quotation_of (@pair A B) | 0
-  := tApp <% @pair %> [qA; qB].
-#[export] Polymorphic Instance qprod_cps {A B} {qA : quotation_of A} {qB : quotation_of B} : quotation_of (@prod A B) | 0
-  := tApp <% @prod %> [qA; qB].
-#[export] Polymorphic Instance qSome_cps {A} {qA : quotation_of A} : quotation_of (@Some A) | 0
-  := tApp <% @Some %> [qA].
-#[export] Polymorphic Instance qNone_cps {A} {qA : quotation_of A} : quotation_of (@None A) | 0
-  := tApp <% @None %> [qA].
-#[export] Polymorphic Instance qoption_cps {A} {qA : quotation_of A} : quotation_of (@option A) | 0
-  := tApp <% @option %> [qA].
-#[export] Polymorphic Instance qcons_cps {A} {qA : quotation_of A} : quotation_of (@cons A) | 0
-  := tApp <% @cons %> [qA].
-#[export] Polymorphic Instance qnil_cps {A} {qA : quotation_of A} : quotation_of (@nil A) | 0
-  := tApp <% @nil %> [qA].
-#[export] Polymorphic Instance qlist_cps {A} {qA : quotation_of A} : quotation_of (@list A) | 0
-  := tApp <% @list %> [qA].
-
-Polymorphic Definition ground_quotable_of_iffT {A B} {quoteA : ground_quotable A} {qA : quotation_of A} {qB : quotation_of B} (H : A <~> B) {qH : quotation_of H} : ground_quotable B.
-Proof.
-  intro b.
-  change (@quotation_of B (fst H (snd H b))).
-  make_quotation_of_goal ().
-Defined.
-(* Transparent versions *)
-Definition proj1 {A B} (x : A /\ B) : A := ltac:(apply x).
-Definition proj2 {A B} (x : A /\ B) : B := ltac:(apply x).
-Definition ground_quotable_of_iff {A B : Prop} {quoteA : ground_quotable A} {qA : quotation_of A} {qB : quotation_of B} (H : iff A B) {qH : quotation_of H} : ground_quotable B.
-Proof.
-  intro b.
-  change (@quotation_of B (proj1 H (proj2 H b))).
-  exact _.
-Defined.
-Definition quote_neg_of_iffT {A B} {quoteA : ground_quotable (A -> False)} {qA : quotation_of A} {qB : quotation_of B} (H : A <~> B) {qH : quotation_of H} : ground_quotable (B -> False).
-Proof.
-  intro nb.
-  assert (na : A -> False) by (intro a; apply nb, H, a).
-  change (@quotation_of (B -> False) (fun b => na (snd H b))).
-  exact _.
-Defined.
-Definition quote_neg_of_iff {A B : Prop} {quoteA : ground_quotable (~A)} {qA : quotation_of A} {qB : quotation_of B} (H : iff A B) {qH : quotation_of H} : ground_quotable (~B).
-Proof.
-  intro nb.
-  assert (na : ~A) by (intro a; apply nb, H, a).
-  change (@quotation_of (~B) (fun b => na (proj2 H b))).
-  exact _.
-Defined.
-
-Ltac unfold_quotation_of _ :=
-  lazymatch goal with
-  | [ |- @quotation_of ?A ?t ]
-    => first [ progress cbv delta [t]
-             | change (@quotation_of A (transparentify t)) ]
-  end.
-
-(* for universe adjustment with [tmDeclareQuotationOfModule], [tmMakeQuotationOfModule] *)
-#[export] Unset MetaCoq Strict Unquote Universe Mode.
-(* N.B. We need to kludge around COQBUG(https://github.com/coq/coq/issues/17303) in Kernames :-( *)
-Polymorphic Definition tmMakeQuotationOfConstants_gen@{d t u _T _above_u'} {debug:debug_opt} (work_around_coq_bug_17303 : bool) (include_submodule : list ident -> bool) (include_supermodule : list ident -> list ident -> bool) (existing_instance : option hint_locality) (base : modpath) (cs : list global_reference) (tmDoWithDefinition : ident -> forall A : Type@{d}, A -> TemplateMonad@{t u} A) : TemplateMonad@{t u} unit
-  := let warn_bad_ctx c ctx :=
-       (_ <- tmMsg "tmPrepareMakeQuotationOfModule: cannot handle polymorphism";;
-        _ <- tmPrint c;;
-        _ <- tmPrint ctx;;
-        tmReturn tt) in
-     let tmDebugMsg s := (if debug
-                          then tmMsg s
-                          else tmReturn tt) in
-     let tmDebugPrint {T : Type@{_T}} (v : T)
-       := (if debug
-           then tmPrint v
-           else tmReturn tt) in
-     let on_bad_relevance r :=
-       (_ <- tmDebugMsg "skipping irrelevant constant";;
-        _ <- tmDebugPrint r;;
-        tmReturn tt) in
-     let make_qname '(mp, name)
-       (* ideally we'd replace _ with __ so that there can't be any collision, but the utility functions aren't written and we don't need it in practice *)
-       := option_map
-            (fun n => "q" ++ n)%bs
-            match split_common_prefix base mp with
-            | None => if include_supermodule [] []
-                      then Some name
-                      else None
-            | Some (_, (_common, [], [])) => Some name
-            | Some (_, (_common, [], postfix))
-              => if include_submodule postfix
-                 then Some (String.concat "__DOT__" postfix ++ "__" ++ name)
-                 else None
-            | Some (_, (_common, base_postfix, postfix))
-              => if include_supermodule base_postfix postfix
-                 then Some ("__DOT_DOT__" ++ String.concat "__DOT__" base_postfix ++ "__SLASH__" ++ String.concat "__DOT__" postfix ++ "__" ++ name)
-                 else None
-            end%bs in
-     let tmDebugSkipGR '(mp, name) :=
-       _ <- tmDebugMsg ("tmMakeQuotationOfConstants_gen: skipping excluded constant " ++ name);;
-       _ <- tmDebugPrint (split_common_prefix base mp);;
-       ret tt in
-     let make_definition '(name, tyv)
-       := ((let tmTyv := tmRetypeAroundMetaCoqBug853 name tyv in
-            _ <- tmDebugPrint tmTyv;;
-            '{| my_projT1 := ty ; my_projT2 := v |} <- tmTyv;;
-            tmDef_name <- tmEval cbv (@tmDoWithDefinition (name:string));;
-            let tmn := tmDef_name ty v in
-            _ <- tmDebugPrint tmn;;
-            n <- tmn;;
-            _ <- tmDebugMsg "tmMakeQuotationOfConstants_gen: tmQuoteToGlobalReference";;
-            qn <- tmQuoteToGlobalReference n;;
-            tmReturn qn) : TemplateMonad global_reference) in
-     let make_instance p
-       := (match existing_instance return TemplateMonad unit with
-           | Some locality
-             => let tmEx := tmExistingInstance locality p in
-                _ <- tmDebugPrint tmEx;;
-                tmEx
-           | None => tmReturn tt
-           end) in
-     let cs := dedup_grefs cs in
-     cs <- tmEval cbv cs;;
-     _ <- tmDebugMsg "tmMakeQuotationOfConstants_gen: looking up module constants";;
-     ps <- monad_map@{_ _ Set _above_u'}
-             (fun r
-              => _ <- tmDebugMsg "tmMakeQuotationOfConstants_gen: handling";;
-                 _ <- tmDebugPrint r;;
-                 match r with
-                 | ConstRef cr
-                   => match make_qname cr with
-                      | None => tmDebugSkipGR cr
-                      | Some qname
-                        => '(univs, rel) <- tmQuoteConstantUniversesAndRelevance cr false;;
-                           match rel with
-                           | Irrelevant => on_bad_relevance cr
-                           | Relevant
-                             => inst <- match univs with
-                                        | Monomorphic_ctx => tmReturn ([] : Instance.t)
-                                        | (Polymorphic_ctx (univs, constraints)) as ctx
-                                          => _ <- warn_bad_ctx cr ctx;;
-                                             tmReturn ([] : Instance.t)
-                                        end;;
-                                let c := tConst cr inst in
-                                _ <- tmDebugMsg "tmMakeQuotationOfConstants_gen: tmUnquote";;
-                                '{| my_projT1 := cty ; my_projT2 := cv |} <- tmUnquote c;;
-                                _ <- tmDebugMsg "tmMakeQuotationOfConstants_gen: tmUnquote done";;
-                                def <- make_definition
-                                         (qname, if work_around_coq_bug_17303
-                                                 then {| my_projT1 := term ; my_projT2 := c |}
-                                                 else {| my_projT1 := @quotation_of cty cv ; my_projT2 := c |});;
-                                make_instance def
-                           end
-                      end
-                 | IndRef ind
-                   => let '{| inductive_mind := r |} := ind in
-                      match make_qname r with
-                      | None => tmDebugSkipGR r
-                      | Some qname
-                        => inst <- (univs <- tmQuoteInductiveUniverses r;;
-                                    match univs with
-                                    | Monomorphic_ctx => tmReturn ([] : Instance.t)
-                                    | (Polymorphic_ctx (univs, constraints)) as ctx
-                                      => _ <- warn_bad_ctx r ctx;;
-                                         tmReturn ([] : Instance.t)
-                                    end);;
-                           let c := tInd ind inst in
-                           _ <- tmDebugMsg "tmMakeQuotationOfConstants_gen: tmUnquote";;
-                           '{| my_projT1 := cty ; my_projT2 := cv |} <- tmUnquote c;;
-                           _ <- tmDebugMsg "tmMakeQuotationOfConstants_gen: tmUnquote done";;
-                           let tmcty := tmRetypeRelaxSetInCodomain@{t t u} qname cty in
-                           _ <- tmDebugPrint tmcty;;
-                           cty <- tmcty;;
-                           let tmcv := tmObj_magic (B:=cty) cv in
-                           _ <- tmDebugPrint tmcv;;
-                           cv <- tmcv;;
-                           let ty := @inductive_quotation_of cty cv in
-                           let v : ty := {| qinductive := ind ; qinst := inst |} in
-                           def <- make_definition
-                                    (qname, {| my_projT1 := ty ; my_projT2 := v |});;
-                           make_instance def
-                      end
-                 | ConstructRef _ _ | VarRef _ => tmReturn tt
-                 end)
-             cs;;
-     ret tt.
-
-Definition tmMakeQuotationOfConstants {debug:debug_opt} (include_submodule : list ident -> bool) (include_supermodule : list ident -> list ident -> bool) (existing_instance : option hint_locality) (base : modpath) (cs : list global_reference) : TemplateMonad unit
-  := tmMakeQuotationOfConstants_gen false include_submodule include_supermodule existing_instance base cs (fun name ty body => @tmDefinition name ty body).
-
-Definition tmMakeQuotationOfConstantsWorkAroundCoqBug17303 {debug:debug_opt} (include_submodule : list ident -> bool) (include_supermodule : list ident -> list ident -> bool) (base : modpath) (cs : list global_reference) : TemplateMonad unit
-  := tmMakeQuotationOfConstants_gen true include_submodule include_supermodule None base cs (fun name ty body => @tmDefinition name ty body).
-
-Definition tmDeclareQuotationOfConstants {debug:debug_opt} (include_submodule : list ident -> bool) (include_supermodule : list ident -> list ident -> bool) (existing_instance : option hint_locality) (base : modpath) (cs : list global_reference) : TemplateMonad unit
-  := tmMakeQuotationOfConstants_gen false include_submodule include_supermodule existing_instance base cs (fun name ty _ => @tmAxiom name ty).
-
-Variant submodule_inclusion := only_toplevel | all_submodules_except (_ : list (list ident)) | toplevel_and_submodules (_ : list (list ident)) | everything.
-
-#[local] Typeclasses Transparent ident IdentOT.t.
-Definition is_submodule_of (super : list ident) (sub : list ident) : bool
-  := firstn #|super| sub == super.
-Definition is_supermodule_of (sub : list ident) (super : list ident) : bool
-  := is_submodule_of super sub.
-Definition include_submodule_of_submodule_inclusion (si : submodule_inclusion) : list ident -> bool
-  := match si with
-     | only_toplevel => fun _ => false
-     | all_submodules_except ls => fun i => negb (existsb (is_supermodule_of i) ls)
-     | toplevel_and_submodules ls => fun i => existsb (is_supermodule_of i) ls
-     | everything => fun _ => true
-     end.
-Definition include_supermodule_of_submodule_inclusion (si : submodule_inclusion) : list ident -> list ident -> bool
-  := match si with
-     | everything => fun _ _ => true
-     | _ => fun _ _ => false
-     end.
-
-Definition tmMakeQuotationOfModule {debug:debug_opt} (include_submodule : submodule_inclusion) (existing_instance : option hint_locality) (m : qualid) : TemplateMonad _
-  := cs <- tmQuoteModule m;;
-     base <- tmLocateModule1 m;;
-     let include_supermodule := include_supermodule_of_submodule_inclusion include_submodule in
-     let include_submodule := include_submodule_of_submodule_inclusion include_submodule in
-     tmMakeQuotationOfConstants include_submodule include_supermodule existing_instance base cs.
-Global Arguments tmMakeQuotationOfModule {_%bool} _ _ _%bs.
-
-Definition tmMakeQuotationOfModuleWorkAroundCoqBug17303 {debug:debug_opt} (include_submodule : submodule_inclusion) (m : qualid) : TemplateMonad _
-  := cs <- tmQuoteModule m;;
-     base <- tmLocateModule1 m;;
-     let include_supermodule := include_supermodule_of_submodule_inclusion include_submodule in
-     let include_submodule := include_submodule_of_submodule_inclusion include_submodule in
-     tmMakeQuotationOfConstantsWorkAroundCoqBug17303 include_submodule include_supermodule base cs.
-Global Arguments tmMakeQuotationOfModuleWorkAroundCoqBug17303 {_%bool} _ _%bs.
-
-Definition tmDeclareQuotationOfModule {debug:debug_opt} (include_submodule : submodule_inclusion) (existing_instance : option hint_locality) (m : qualid) : TemplateMonad _
-  := cs <- tmQuoteModule m;;
-     base <- tmLocateModule1 m;;
-     let include_supermodule := include_supermodule_of_submodule_inclusion include_submodule in
-     let include_submodule := include_submodule_of_submodule_inclusion include_submodule in
-     tmDeclareQuotationOfConstants include_submodule include_supermodule existing_instance base cs.
-Global Arguments tmDeclareQuotationOfModule {_%bool} _ _ _%bs.
-
-(*
-Require Import MSetPositive.
-Instance: debug_opt := true.
-MetaCoq Run (tmMakeQuotationOfModule None "Coq.MSets.MSetPositive.PositiveSet"%bs).
-*)
